books/xdoc/top.lisp
@@ -18,516 +18,81 @@
 ;
 ; Original author: Jared Davis <jared@centtech.com>
 
+
+; top.lisp -- most end users should include this book directly.  If you are
+; new to xdoc, you can try running:
+;
+;  (include-book "xdoc/top" :dir :system)
+;  :xdoc xdoc
+
 (in-package "XDOC")
-(include-book "defxdoc")
-(include-book "save")
-
-(defxdoc xdoc
-  :short "<em>XDOC</em> is a new mechanism for documenting ACL2 libraries, and
-is intended as a replacement for ACL2 facilities such as <tt>defdoc</tt>,
-<tt>:doc</tt>, and so on.")
-
-
-(defxdoc defxdoc
-  :parents (xdoc)
-  :short "Add some new documentation to the @(see xdoc) database."
-
-  :long "<p><tt>Defxdoc</tt> is the XDOC alternative to ACL2's built-in
-<tt>defdoc</tt> command.  To use <tt>defxdoc</tt>, the first step is to include
-the <tt>xdoc/defxdoc</tt> book, e.g.,</p>
-
-<code>
-(include-book \"xdoc/defxdoc\" :dir :system)
-</code>
-
-<p>This book is quite minimal so that it will not interfere with your
-libraries.  Once the book is loaded, you can begin documenting your functions
-using the <tt>defxdoc</tt> command.</p>
-
-<code>
-(defxdoc name
-  :parents (topic1 topic2 ...)
-  :short \"short description\"
-  :long \"longer description\")
-</code>
-
-<p>All of the keyword arguments are optional.</p>
-
-<ul>
-
- <li><tt>name</tt> is the name of this documentation topic, and should be a
-symbol.</li>
-
- <li><tt>parents</tt> let you associate this documentation with other topics.
-A topic can have many parents, but circular parents are not allowed and will
-lead to errors when generating documentation.</li>
-
- <li><tt>short</tt> should be a short description of this topic and should be
-suitable for inlining in other pages.  (For instance, it is displayed in the
-full index, and as \"hover\" text in the listing frames.)</li>
-
- <li><tt>long</tt> should be the full, detailed documentation for this
-topic.</li>
-
-</ul>
-
-<p>The <tt>short</tt> and <tt>long</tt> strings may be written using the XDOC
-@(see markup) language, and may also use @(see preprocessor) commands to insert
-function definitions, theorems, topic links, and so on.</p>
-
-<h3>Notes for Advanced Users</h3>
-
-<p>XDOC just stores its documentation in an ordinary ACL2 table, so if you
-want to do something like automatically generate documentation from macros,
-you might decide to bypass @(srclink defxdoc) and just manipulate the table
-directly.</p>")
-
-
-
-(defxdoc markup
-  :parents (defxdoc)
-  :short "XDOC documentation strings are mainly written in a simple XML markup
-language.  XML is basically similar to HTML, but is very insistent that tags
-begin and end in balance."
-
-  :long "<h3>Formatting Text</h3>
-
-<p>Various tags allow you to control the font:</p>
-<ul>
- <li><b>&lt;b&gt;bold&lt;/b&gt;</b></li>
- <li><i>&lt;i&gt;italics&lt;/i&gt;</i></li>
- <li><u>&lt;u&gt;underline&lt;/u&gt;</u></li>
- <li><tt>&lt;tt&gt;typewriter text&lt;/tt&gt;</tt></li>
- <li><color rgb=\"#ff0000\">&lt;color rgb=&quot;#ff0000&quot;&gt;colored text&lt;/color&gt;</color></li>
- <li><sf>&lt;sf&gt;sans-serif&lt;/sf&gt;</sf></li>
-</ul>
-
-<h3>Displaying Source Code</h3>
-
-<p>The <tt>&lt;tt&gt;</tt> tag is intended for short, inline pieces of code,
-such as <tt>(+ 1 x)</tt>.  In contrast, the <tt>&lt;code&gt;</tt> tag is
-intended for longer code examples that should be indented and \"preformatted,\"
-i.e., newlines and spaces should be preserved.</p>
-
-<p>Note that the @(see preprocessor) allows you to insert function definitions,
-theorems, etc., from the ACL2 world, so typically <tt>&lt;code&gt;</tt> is only
-needed for examples. </p>
-
-<h3>Adding Hyperlinks</h3>
-
-<p><i>Internal links</i> between documentation topics and <i>Emacs
-tags-search links</i> into the source code are handled by the @(see
-preprocessor).</p>
-
-<p>It is also posible to add <i>external links</i> to web pages with ordinary
-HTML-style links, e.g.,</p>
-
-<code>
-&lt;a href=\"http://www.centtech.com/\"&gt;Centaur Technology&lt;/a&gt;
-</code>
-
-<p>Produces a link to <a href=\"http://www.centtech.com/\">Centaur
-Technology</a>.</p>
-
-
-<h3>Structuring Documents</h3>
-
-<p>Paragraphs should begin and end with the <tt>&lt;p&gt;</tt> tag.  (You can also
-do individual line breaks with <tt>&lt;br/&gt;</tt>.)</p>
-
-<p>For section headings, <tt>&lt;h1&gt;</tt> creates the biggest heading,
-<tt>&lt;h2&gt;</tt> the next biggest, and so on.  The smallest heading is
-<tt>&lt;h5&gt;</tt>.</p>
-
-<p>Bulleted and numbered lists work as in HTML.  The list itself begins with
-<tt>&lt;ul&gt;</tt> (for bulleted lists) or <tt>&lt;ol&gt;</tt> (for numbered lists).
-Each list element is an <tt>&lt;li&gt;</tt> tag.  For instance,</p>
-
-<code>
-&lt;ul&gt;
-  &lt;li&gt;one&lt;/li&gt;
-  &lt;li&gt;two&lt;/li&gt;
-  &lt;li&gt;three&lt;/li&gt;
-&lt;/ul&gt;
-</code>
-
-<p>Produces:</p>
-
-<box>
-<ul>
-  <li>one</li>
-  <li>two</li>
-  <li>three</li>
-</ul>
-</box>
-
-<p>You can also use definition lists, which are comprised
-of <tt>&lt;dl&gt;</tt>, <tt>&lt;dt&gt;</tt>, and <tt>&lt;dd&gt;</tt> tags.  For
-instance,</p>
-
-<code>
-&lt;dl&gt;
-  &lt;dt&gt;Inputs&lt;/dt&gt;
-  &lt;dd&gt;&lt;tt&gt;x&lt;/tt&gt;, the list we are traversing&lt;/dd&gt;
-  &lt;dd&gt;&lt;tt&gt;max&lt;/tt&gt;, limit on how many we can accumulate&lt;/dd&gt;
-  &lt;dd&gt;&lt;tt&gt;acc&lt;/tt&gt;, accumulator for our results&lt;/dd&gt;
-&lt;/dl&gt;
-</code>
-
-<p>Produces:</p>
-
-<box>
-<dl>
-  <dt>Inputs</dt>
-  <dd><tt>x</tt>, the list we are traversing</dd>
-  <dd><tt>max</tt>, limit on how many we can accumulate</dd>
-  <dd><tt>acc</tt>, accumulator for our results</dd>
-</dl>
-</box>
-
-<p>These framed boxes are generated with the <tt>&lt;box&gt;</tt> tag.</p>")
-
-
-(defxdoc preprocessor
-  :parents (defxdoc)
-  :short "In addition to its @(see markup) language, XDOC includes a
-preprocessor which can be used to interpret certain directives of the form
-<tt>@@(...)</tt>."
-
-  :long "<h3>Functions and Theorems</h3>
-
-<p>To insert function definitions (or pieces of definitions) into your
-documentation, you can use:</p>
-
-<ul>
- <li><tt>@@(def fn)</tt>, expands to the definition of the function (or macro)
-     <i>fn</i></li>
- <li><tt>@@(body fn)</tt>, just the body of <i>fn</i></li>
- <li><tt>@@(formals fn)</tt>, just the formals of <i>fn</i></li>
- <li><tt>@@(measure fn)</tt>, just the measure of <i>fn</i></li>
- <li><tt>@@(call fn)</tt>, a generic function call of <i>fn</i></li>
-</ul>
-
-<p>We expect that <tt>def</tt> and <tt>body</tt> directives will
-expand to large code fragments, so they are automatically wrapped in
-<tt>&lt;code&gt;</tt> blocks and other formatting.</p>
-
-<p>The <tt>call</tt> directive is automatically wrapped in &lt;tt&gt;
-tags, i.e., <tt>@@(call fib)</tt> might become &lt;tt&gt;(fib x)&lt;/tt&gt;.
-An alternative is to use <tt>@@(ccall fib)</tt>, for \"code call,\" which
-inserts &lt;code&gt; tags instead.</p>
-
-<p>The other directives just become plain text, and you can wrap whatever
-formatting commands you like around them and use them inline in paragraphs,
-etc.</p>
-
-<p>You can also insert theorems:</p>
-
-<ul>
- <li><tt>@@(thm name)</tt>, expands to the statement of the theorem <i>name</i></li>
-</ul>
-
-<p>As with <tt>def</tt> and <tt>body</tt> directives, <tt>thm</tt> directives
-automatically insert <tt>&lt;code&gt;</tt> blocks.</p>
-
-<h3>Documentation Links</h3>
-
-<p>The easiest way to link between topics is to use <tt>@@(see name)</tt>,
-which expands into a link to <tt>name</tt>.  The text shown to the reader is
-just the name of the topic, in lower case.  Note also that <tt>@@(csee
-name)</tt> can be used for links whose first letter should be capitalized.</p>
-
-<p>For most purposes, <tt>@@(see name)</tt> is adequate and it is also
-recommended.  Finer-grained control (e.g., changing the link text) is also
-possible, but requires some considerations for mangling file names, etc.
-Basically, <tt>@@(see name)</tt> expands to:</p>
-
-<code>
-&lt;see topic=\"mangled-topic-name\"&gt;printed-topic-name&lt;/see&gt;
-</code>
-
-<p>Where:</p>
-
-<ul>
-<li><tt>mangled-topic-name</tt> is a canonical, url and file-name friendly
-   mangling of <tt>name</tt>'s package and symbol names, and</li>
-
-<li><tt>printed-topic-name</tt> is an XML-escaped (i.e., \"&lt;\" becomes
-   \"&amp;lt;\") variant of <tt>name</tt> which, depending on the package of the
-   current topic's name, may or may not include the package portion of
-   <tt>name</tt>.</li>
-</ul>
-
-<p>So, to support custom links, we provide</p>
-
-<ul>
- <li><tt>@@(url name)</tt>, which expands to <tt>mangled-topic-name</tt></li>
- <li><tt>@@(sym name)</tt>, which expands to <tt>printed-topic-name</tt></li>
- <li><tt>@@(csym name)</tt>, like <tt>sym</tt>, but with the first letter capitalized</li>
-</ul>
-
-<p>and these can be used to form a custom <tt>&lt;see&gt;</tt> tag.</p>
-
-
-<h3>Emacs Links</h3>
-
-<p>The <tt>@@(srclink name)</tt> directive inserts a source-code link for users
-who have configured their web browser as described in @(see
-emacs-web-integration).</p>
-
-<p>It is often unnecessary to use <tt>srclink</tt> directly, because these
-links are automatically inserted by the <tt>@@(def fn)</tt> and <tt>@@(thm
-foo)</tt> directives.  One good reason to use <tt>srclink</tt> is to link to
-macros like @(srclink defxdoc), which often are written using backquote and
-hence do not display nicely.</p>
-
-<p>Source links are sometimes inappropriate, e.g., for definitions or theorems
-that are generated by macros.  You can suppress the automatic source links on
-<tt>def</tt> and <tt>thm</tt> commands by using <tt>@@(gdef fn)</tt> or
-<tt>@@(gthm foo)</tt> instead, which stand for \"generated def\" and
-\"generated thm.\"</p>
-
-
-
-<h3>Escaping of @</h3>
-
-<p>Since <tt>@@(</tt> is intercepted by the preprocessor, you may occasionally
-need to escape it.  You can write <tt>@@@@</tt> to generate a single <tt>@</tt>
-sign.</p>
-
-<p>Besides <tt>@@(</tt> and <tt>@@@@</tt>, the preprocessor leaves any other uses
-of <tt>@</tt> in tact.  So, most uses of <tt>@</tt>, such as in email
-addresses, do not need to be escaped.</p>")
-
-
-
-(defxdoc manual-generation
-  :parents (xdoc)
-
-  :short "To construct a manual for your library, the XDOC database can be
-saved into <tt>.xml</tt> files, which can then be translated into HTML and
-other formats."
-
-  :long "<p>The <tt>defxdoc</tt> command only adds documentation to the
-database.  To actually generate a nice manual for your library, there are two
-steps.</p>
-
-<ol>
-  <li>Save the XDOC database into <tt>.xml</tt> files, then</li>
-  <li>Use an XSLT transformer to convert the files into HTML, TEXT, or some
-other format.</li>
-</ol>
-
-<p>Both of these topics are covered here.</p>
-
-<h3>Saving the XML Files</h3>
-
-<p>The first step in generating a manual is to save the XDOC database into XML
-files.  The basic commands for doing this are:</p>
-
-<code>
-;; 1. Load your own library.
-(include-book \"your-library\")
-
-;; 2. Load the save command.
-(include-book \"xdoc/save\" :dir :system)
-
-;; 3. Run the save command to produce the .xml files.
-(xdoc::save &lt;dir&gt;)
-</code>
-
-<p>where <tt>&lt;dir&gt;</tt> is the directory you want the documentation
-written to.  Note that:</p>
-
-<ul>
-  <li> <tt>&lt;dir&gt;</tt> must already exist in order for
-this to work, and</li>
-  <li> files in <tt>dir</tt> <color rgb=\"#ff0000\">may be overwritten!</color></li>
-</ul>
-
-<h3>Transforming the XML Files</h3>
-
-<p>Once the documentation has been saved, you can view the resulting <tt>.xml</tt>
-files directly in a web browser.</p>
-
-<p>Future work includes providing tools to translate these XML files into other
-formats, and for viewing them with some kind of <tt>:xdoc</tt> command from
-directly within ACL2.</p>")
-
-
-(defxdoc emacs-web-integration
-  :parents (xdoc)
-
-  :short "Instructions for integrating XDOC web pages with Emacs."
-
-  :long "<p>@(csee preprocessor) directives such as <tt>@@(def
-get-xdoc-table)</tt> result in the introduction of special links for Emacs.
-With a little work, you can configure your web browser so that clicking on
-these links will cause Emacs to directly open up the appropriate source file
-and jump to the named function.  Here is what such a link looks like:</p>
-
-@(def get-xdoc-table)
-
-<p>How does this work?</p>
-
-<ul>
-
- <li>Emacs links are actually links to <tt>xdoc-link</tt> files.</li>
-
- <li>We instruct your web browser to send these files to Emacs.</li>
-
- <li>We instruct Emacs to carry out a tags search instead of loading these
-files.</li>
-
-</ul>
-
-<p>The net effect is that clicking on these links will send you directly
-to the desired function in the source code.  This is really cool, and it
-is not too hard to set up.</p>
-
-
-<h2>Configuring Emacs</h2>
-
-<h4>Loading the XDOC Elisp</h4>
-
-<p>The XDOC directory includes a file called <tt>xdoc.el</tt>, which tells
-emacs what to do with these <tt>xdoc-link</tt> files.  To tell emacs to load
-this file at startup, you can just add a command to your <tt>.emacs</tt> file
-such as:</p>
-
-<code>
-(load \"/path/to/xdoc/xdoc.el\")
-</code>
-
-
-<h4>Managing your TAGS tables</h4>
-
-<p>For emacs to make sense of the links you follow, it will need to have the
-appropriate <a
-href=\"http://www.gnu.org/software/emacs/manual/html_node/emacs/Tags.html\">tags
-tables</a> loaded for all of the libraries you are using.</p>
-
-<p>If you aren't familiar with tags, you basically just need to:</p>
-<ul>
-  <li>Occasionally generate <tt>TAGS</tt> files for your libraries,
-      using the command <tt>etags *.lisp</tt>.</li>
-
-  <li>Tell Emacs to \"visit\" these tags tables with
-      <tt>visit-tags-table</tt>.</li>
-</ul>
-
-<p>Here's how I do it:</p>
-
-<ul>
-
-<li>I add a <tt>TAGS</tt> target to my Makefiles, so that when I build my
-library the <tt>etags *.lisp</tt> command is re-run and the <tt>TAGS</tt>
-file is kept up to date.  The Makefile syntax is:
-
-<code>
-TAGS: $(wildcard *.lisp)
-      etags *.lisp
-</code></li>
-
-<li>Then, in my <tt>.emacs</tt> file, I have a series of commands like the
-following:
-
-<code>
-(ignore-errors (visit-tags-table \"/path/to/acl2/TAGS\"))
-(ignore-errors (visit-tags-table \"/path/to/acl2/books/xdoc/TAGS\"))
-(ignore-errors (visit-tags-table \"/path/to/my/stuff/TAGS\"))
-</code>
-
-This ensures that the relevant <tt>TAGS</tt> files are loaded every time I
-start Emacs.  The use of <tt>ignore-errors</tt> prevents Emacs from complaining
-if one of these <tt>TAGS</tt> files was deleted in a \"make clean\" or
-similar.</li>
-
-<li>One final addition to the <tt>.emacs</tt> file is:
-
-<code>
-(setq tags-revert-without-query t)
-</code>
-
-which tells Emacs to go ahead and reload these files when they are rebuilt
-by Make, instead of prompting you if you want to reload them.</li>
-
-</ul>
-
-
-<h4>Setting up Emacsclient (recommended)</h4>
-
-<p>You can set things up so that links open up in <b>new instances</b> of
-Emacs, or in <b>new buffers</b> of an already-running Emacs.  If you want
-everything to open up in a new instance of Emacs, you can skip this section.
-But I greatly prefer to use a single Emacs for everything, and just have links
-open up in new buffers.</p>
-
-<p>This is quite easy.  First, add <tt>(server-start)</tt> to your
-<tt>.emacs</tt> file and restart Emacs.</p>
-
-<p>Next, to ensure everything is working properly, launch a separate terminal
-and type:</p>
-
-<code>
-emacsclient --no-wait my-file
-</code>
-
-<p>If all is well, <tt>my-file</tt> will be loaded into your already-running
-emacs as a new buffer.</p>
-
-
-
-<h2>Configuring the Web Browser</h2>
-
-<p>The last thing we need to do is instruct your web browser to send
-<tt>xdoc-link</tt> files to Emacs.  How this is done depends on your
-web browser.</p>
-
-<h4>Firefox (works)</h4>
-
-<p><b>Note:</b> I have not yet found a way to get Firefox to call
-<tt>emacsclient</tt> with the <tt>--no-wait</tt> option.  To work around this,
-I wrote a trivial script called <tt>emacsclient-wrapper.sh</tt>, which is
-included in the XDOC directory.</p>
-
-<ol>
-
-<li>Install the <a
-href=\"https://addons.mozilla.org/en-US/firefox/addon/4498\">MIME Edit</a>
-firefox plugin.  This is quite easy, but requires firefox to be restarted.</li>
-
-<li>Use MIME-EDIT to tell firefox to give <tt>.xdoc-link</tt> files to emacs:
-
-<ul>
-  <li>Choose (from the menu bar): <tt>Tools</tt>, <tt>MIME Edit</tt></li>
-  <li>Pick the <tt>Edit</tt> tab</li>
-  <li>Click <tt>New Type</tt></li>
-  <li>MIME Type: <u>application/acl2-xdoc-link</u></li>
-  <li>Description: <u>Link to ACL2 Source Code</u></li>
-  <li>Extension: <u>xdoc-link</u></li>
-  <li>When encountered, open file with <u>/path/to/emacsclient-wrapper.sh</u></li>
-</ul>
-
-</li>
-</ol>
-
-<h4>Safari (not working yet)</h4>
-
-<p>I am mainly unfamiliar with MacOS, so perhaps someone can figure this out.
-I did not see any mechanism to edit MIME types directly within Safari.  However,
-there is a free program called <a href=\"http://mac.clauss-net.de/misfox/\">MisFox</a>
-program which allows you to set up file mappings.  But its \"choose\" dialog for
-picking the program refuses to accept <tt>emacsclient</tt> or a wrapper script, for
-whatever reason that I do not understand.</p>
-
-<h4>Internet Explorer</h4>
-
-<p>BOZO figure this out</p>
-
-
-
-")
-
-
+(include-book "base")
+; (depends-on "save.cert")
+; (depends-on "display.cert")
+; (depends-on "topics.cert")
+; (depends-on "defxdoc-raw.cert")
+; (depends-on "mkdir-raw.cert")
+
+(make-event `(defconst *xdoc-dir/save*
+               ,(acl2::extend-pathname *xdoc-dir* "save" state)))
+(make-event `(defconst *xdoc-dir/display*
+               ,(acl2::extend-pathname *xdoc-dir* "display" state)))
+(make-event `(defconst *xdoc-dir/topics*
+               ,(acl2::extend-pathname *xdoc-dir* "topics" state)))
+(make-event `(defconst *xdoc-dir/defxdoc-raw*
+               ,(acl2::extend-pathname *xdoc-dir* "defxdoc-raw" state)))
+(make-event `(defconst *xdoc-dir/mkdir-raw*
+               ,(acl2::extend-pathname *xdoc-dir* "mkdir-raw" state)))
+
+
+(defmacro xdoc (name)
+  (declare (xargs :guard (or (symbolp name)
+                             (and (quotep name)
+                                  (symbolp (unquote name))))))
+  (let ((name (if (symbolp name)
+                  name
+                (unquote name))))
+    `(with-output :off (summary event)
+       (progn
+         (include-book ,*xdoc-dir/defxdoc-raw* :ttags :all)
+         (include-book ,*xdoc-dir/topics*)
+         (include-book ,*xdoc-dir/display*)
+         (make-event
+          (b* (((mv all-xdoc-topics state) (all-xdoc-topics state))
+               ((mv & & state) (colon-xdoc-fn ',name nil all-xdoc-topics state)))
+            (value '(value-triple :invisible))))))))
+
+(defmacro xdoc! (name)
+  (declare (xargs :guard (or (symbolp name)
+                             (and (quotep name)
+                                  (symbolp (unquote name))))))
+  (let ((name (if (symbolp name)
+                  name
+                (unquote name))))
+    `(with-output :off (summary event)
+       (progn
+         (include-book ,*xdoc-dir/defxdoc-raw* :ttags :all)
+         (include-book ,*xdoc-dir/topics*)
+         (include-book ,*xdoc-dir/display*)
+         (make-event
+          (b* (((mv all-xdoc-topics state) (all-xdoc-topics state))
+               ((mv & & state) (colon-xdoc-fn ',name t all-xdoc-topics state)))
+            (value '(value-triple :invisible))))))))
+
+(defmacro save (dir &key (index-pkg 'acl2::foo))
+  `(progn
+     (include-book ,*xdoc-dir/defxdoc-raw* :ttags :all)
+     (include-book ,*xdoc-dir/mkdir-raw* :ttags :all)
+     (include-book ,*xdoc-dir/topics*)
+     (include-book ,*xdoc-dir/save*)
+
+     ;; ugh, stupid stupid writes-ok stupidity
+     (defttag :xdoc)
+     (remove-untouchable acl2::writes-okp nil)
+
+     (make-event
+      (b* (((mv all-xdoc-topics state) (all-xdoc-topics state))
+           ((mv & & state) (assign acl2::writes-okp t))
+           (state (save-topics all-xdoc-topics ,dir ',index-pkg state)))
+        (value '(value-triple :invisible))))))
 
