books/xdoc/parse-xml.lisp
@@ -1,0 +1,363 @@
+; XDOC Documentation System for ACL2
+; Copyright (C) 2009-2010 Centaur Technology
+;
+; Contact:
+;   Centaur Technology Formal Verification Group
+;   7600-C N. Capital of Texas Highway, Suite 300, Austin, TX 78731, USA.
+;   http://www.centtech.com/
+;
+; This program is free software; you can redistribute it and/or modify it under
+; the terms of the GNU General Public License as published by the Free Software
+; Foundation; either version 2 of the License, or (at your option) any later
+; version.  This program is distributed in the hope that it will be useful but
+; WITHOUT ANY WARRANTY; without even the implied warranty of MERCHANTABILITY or
+; FITNESS FOR A PARTICULAR PURPOSE.  See the GNU General Public License for
+; more details.  You should have received a copy of the GNU General Public
+; License along with this program; if not, write to the Free Software
+; Foundation, Inc., 51 Franklin Street, Suite 500, Boston, MA 02110-1335, USA.
+;
+; Original author: Jared Davis <jared@centtech.com>
+
+(in-package "XDOC")
+(include-book "preprocess")
+(set-state-ok t)
+(program)
+
+
+; (PARSE-XML X) --> (MV ERR TOKENS)
+;
+; This is an extremely primitive XML lexer.  It is incomplete, doesn't support
+; unicode, and probably is dead wrong as far as the XML standard is concerned.
+; But, it's adequate for XDOC stuff.
+;
+; X should be an XML-formatted string (with no preprocessor stuff).  We break
+; it into a list of tokens, which may be any of the following:
+;
+;    (:OPEN STR ALIST) represents <tag [... atts ...]>
+;
+;       - STR is a string that is the tag name, e.g., "p" for <p>
+;
+;       - ALIST is an alist of the attribute.  Each entry is either:
+;            (KEY-STR . VAL-STR)   for ordinary key="val" style atts
+;            (KEY-STR . NIL)       for value-free atts like <hr noshade>
+;
+;    (:CLOSE STR) represents </tag>
+;
+;       - STR is a string that is the tag name, e.g., "p" for </p>
+;
+;    (:TEXT STR) represents ordinary text
+;
+;       - STR is the contents of the text.  This is ordinary text with no
+;         embedded tags or entities.
+;
+;    (:ENTITY TYPE) represents entities like &amp;
+;
+;      - TYPE is :AMP, :LT, :GT, :APOS, or :NBSP
+
+(defconst *nls* (coerce (list #\Newline) 'string))
+
+(defun read-until (x n xl stop-chars acc)
+  ;; Accumulate chars until one of the stop-chars is seen
+  "Returns (MV FOUNDP N ACC)"
+  (b* (((when (>= n xl))
+        (mv nil n acc))
+       (char-n (char x n))
+       ((when (member char-n stop-chars))
+        (mv t n acc)))
+    (read-until x (+ 1 n) xl stop-chars (cons char-n acc))))
+
+(defun read-name-aux (x n xl acc)
+  ;; For attribute/tag names.  We just expect alphanumeric characters.  This is
+  ;; probably horribly wrong as far as the XML spec is concerned, but should be
+  ;; reasonable for all the tag and attribute names in xdoc.
+  "Returns (MV N ACC)"
+  (b* (((when (>= n xl))
+        (mv n acc))
+       (char-n (char x n))
+       ((when (or (and (char<= #\a char-n) (char<= char-n #\z))
+                  (and (char<= #\Z char-n) (char<= char-n #\Z))
+                  (and (char<= #\0 char-n) (char<= char-n #\9))
+                  (eql char-n #\_)
+                  (eql char-n #\-)
+                  ))
+        (read-name-aux x (+ 1 n) xl (cons char-n acc))))
+    (mv n acc)))
+
+(defun read-name (x n xl)
+  ;; Try to read an attribute/tag name at the current spot.
+  "Returns (MV ERR N NAME-STR)"
+  (b* (((mv n rchars)
+        (read-name-aux x n xl nil))
+       ((unless (consp rchars))
+        (mv (str::cat "Expected a name, but found unexpected character "
+                      (coerce (list (char x n)) 'string) *nls*
+                      "Nearby text: {" (error-context x n xl) "}" *nls*)
+            n nil))
+       (str (reverse (coerce rchars 'string))))
+    (mv nil n str)))
+
+(defun read-attrval (x n xl)
+  ;; Try to read "value" or 'value' at the current spot.
+  "Returns (MV ERR N VAL-STR)"
+  (b* ((saved-n n)
+       (quote-char (char x n))
+       ((unless (or (eql quote-char #\")
+                    (eql quote-char #\')))
+        (mv (str::cat "Expected value to start with a quote, but found "
+                      (coerce (list (char x n)) 'string) *nls*
+                      "Nearby text: {" (error-context x n xl) "}" *nls*)
+            n nil))
+       (n (+ 1 n)) ;; eat the quote-char
+       ((mv found-endp n chars)
+        (read-until x n xl (list quote-char) nil))
+       ((unless found-endp)
+        (mv (str::cat "Attribute value never ends." *nls*
+                      "Nearby text: {" (error-context x saved-n xl) "}" *nls*)
+            n nil))
+       (n (+ n 1)) ;; eat the closing quote-char
+       (val-str (reverse (coerce chars 'string))))
+    (mv nil n val-str)))
+
+(defun read-tag-attributes (x n xl tag-start-n atts)
+  ;; Assumes "<foo" and perhaps some attributes have just been read.
+  ;; Reads through the closing > or />, setting CLOSEP=T if we read />
+  ;; as in <br/>.
+  "Returns (MV ERR N ATTS CLOSEP)"
+  (b* ((n (skip-past-ws x n xl))
+       ((when (>= n xl))
+        (mv (str::cat "Tag never closes." *nls*
+                      "Nearby text: {" (error-context x tag-start-n xl) "}" *nls*)
+            n nil nil))
+       ((when (eql (char x n) #\>))
+        ;; End of tag via >
+        (mv nil (+ 1 n) atts nil))
+       ((when (eql (char x n) #\/))
+        ;; It had better be />.
+        (b* ((n (+ 1 n))
+             ((unless (and (< n xl)
+                           (eql (char x n) #\>)))
+              (mv (str::cat "Stray / in tag." *nls*
+                            "Nearby text: {" (error-context x tag-start-n xl) "}" *nls*)
+                  n nil nil)))
+          (mv nil (+ 1 n) atts t)))
+       ;; We should now be at the start of some new attribute.
+       ((mv err n key1) (read-name x n xl))
+       ((when err)
+        (mv err n nil nil))
+       (n (skip-past-ws x n xl))
+       ((when (>= n xl))
+        (mv (str::cat "Tag never closes." *nls*
+                      "Nearby text: {" (error-context x tag-start-n xl) "}" *nls*)
+            n nil nil))
+       ((unless (eql (char x n) #\=))
+        ;; I guess this is okay for things like "noshade" that don't have an
+        ;; associated value.
+        (read-tag-attributes x n xl tag-start-n (acons key1 nil atts)))
+       (n (+ n 1)) ;; eat the =
+       (n (skip-past-ws x n xl))
+       ((mv err n val1) (read-attrval x n xl))
+       ((when err)
+        (mv err n nil nil)))
+    (read-tag-attributes x n xl tag-start-n (acons key1 val1 atts))))
+
+(defun read-close-tag (x n xl)
+  ;; Assumes </ has just been read.
+  ;; Reads through the closing >.
+  "Returns (MV ERR N TOKEN-LIST)"
+  (b* ((saved-n n)
+       (n (skip-past-ws x n xl))
+       ((mv err n name) (read-name x n xl))
+       ((when err)
+        (mv err n nil))
+       (n (skip-past-ws x n xl))
+       ((unless (eql (char x n) #\>))
+        (mv (str::cat "Invalid closing tag." *nls*
+                      "Nearby text: {" (error-context x saved-n xl) "}" *nls*)
+            n nil))
+       (n (+ 1 n)) ;; eat the final >
+       (close (list :CLOSE name)))
+    (mv nil n (list close))))
+
+(defun skip-declaration (x n xl start-n)
+  ;; Read through ?>
+  "Returns (MV ERR N NIL)"
+  (b* (((when (>= (- n 1) xl))
+        (mv (str::cat "<? ... ?> declaration never closes." *nls*
+                      "Nearby text: {" (error-context x start-n xl) "}" *nls*)
+            n nil))
+       ((unless (and (eql (char x n) #\?)
+                     (eql (char x (+ n 1)) #\>)))
+        (skip-declaration x (+ n 1) xl start-n)))
+    (mv nil (+ n 2) nil)))
+
+(defun read-tag (x n xl)
+  ;; Assumes (char x n) is "<"
+  "Returns (MV ERR N TOKEN-LIST)"
+  (b* ((tag-start-n n)
+       (n (+ 1 n))
+       (n (skip-past-ws x n xl))
+       ((when (>= n xl))
+        (mv (str::cat "Tag never closes." *nls*
+                      "Nearby text: {" (error-context x tag-start-n xl) "}" *nls*)
+            n nil))
+       ((when (eql (char x n) #\?))
+        (skip-declaration x n xl tag-start-n))
+       ((when (eql (char x n) #\/))
+        (read-close-tag x (+ 1 n) xl))
+       ;; Else, it's an opening tag.  This should be its name.
+       ((mv err n name)
+        (read-name x n xl))
+       ((when err)
+        (mv err n nil))
+       ((mv err n atts closep)
+        (read-tag-attributes x n xl tag-start-n nil))
+       ((when err)
+        (mv err n nil))
+       (open (list :OPEN name (reverse atts)))
+       ((when (not closep))
+        (mv nil n (list open)))
+       (close (list :CLOSE name)))
+    (mv nil n (list open close))))
+
+(defun read-entity (x n xl)
+  ;; Assumes (char x n) is "&"
+  "Returns (MV ERR N TOK)"
+  (b* ((saved-n n)
+       (n (+ 1 n)) ;; eat the &
+       ((mv foundp n rchars)
+        (read-until x n xl (list #\;) nil))
+       ((unless foundp)
+        (mv (str::cat "Entity does not have a closing semicolon." *nls*
+                      "Nearby text: {" (error-context x saved-n xl) "}" *nls*)
+            n nil))
+       (n (+ 1 n)) ;; eat the ;
+       (str (reverse (coerce rchars 'string)))
+       ((when (equal str "amp"))  (mv nil n '(:ENTITY :AMP)))
+       ((when (equal str "lt"))   (mv nil n '(:ENTITY :LT)))
+       ((when (equal str "gt"))   (mv nil n '(:ENTITY :GT)))
+       ((when (equal str "quot")) (mv nil n '(:ENTITY :QUOT)))
+       ((when (equal str "apos")) (mv nil n '(:ENTITY :APOS)))
+       ((when (equal str "nbsp")) (mv nil n '(:ENTITY :NBSP))))
+    (mv (str::cat "Unsupported entity: &" str ";" *nls*
+                  "Nearby text: {" (error-context x xl saved-n) "}" *nls*)
+        n nil)))
+
+(defun parse-xml-aux (x n xl acc)
+  "Returns (MV ERR TOKENS)"
+  (b* (((when (>= n xl))
+        (mv nil acc))
+       (char-n (char x n))
+       ((when (eql char-n #\<))
+        ;; Open/closing tag
+        (b* (((mv err n token-list) (read-tag x n xl))
+             ((when err)
+              (mv err nil))
+             (acc (revappend token-list acc)))
+          (parse-xml-aux x n xl acc)))
+       ((when (eql char-n #\&))
+        ;; Entity
+        (b* (((mv err n token) (read-entity x n xl))
+             ((when err)
+              (mv err nil)))
+          (parse-xml-aux x n xl (cons token acc))))
+       ((when (eql char-n #\>))
+        (mv (str::cat "Stray end-of-tag character '>'" *nls*
+                      "Nearby text: {" (error-context x n xl) "}" *nls*)
+            nil))
+       ;; Otherwise, plain text.
+       ((mv ?foundp n rchars)
+        (read-until x n xl '(#\< #\& #\>) nil))
+       (token (list :TEXT (reverse (coerce rchars 'string)))))
+    (parse-xml-aux x n xl (cons token acc))))
+
+
+; Basic tag balance checking with nice error reporting
+
+(defun opentok-p (x) (eq (first x) :OPEN))
+(defun opentok-name (x) (second x))
+(defun opentok-atts (x) (third x))
+
+(defun closetok-p (x) (eq (first x) :CLOSE))
+(defun closetok-name (x) (second x))
+
+(defun entitytok-p (x) (eq (first x) :ENTITY))
+(defun entitytok-type (x) (second x))
+
+(defun texttok-p (x) (eq (first x) :TEXT))
+(defun texttok-text (x) (second x))
+
+(defun entitytok-as-entity (x)
+  (case (entitytok-type x)
+    (:AMP  "&amp;")
+    (:LT   "&lt;")
+    (:GT   "&gt;")
+    (:QUOT "&quot;")
+    (:APOS "&apos;")
+    (:NBSP "&nbsp;")))
+
+(defun entitytok-as-plaintext (x)
+  (case (entitytok-type x)
+    (:AMP  "&")
+    (:LT   "<")
+    (:GT   ">")
+    (:QUOT "\"")
+    (:APOS "'")
+    (:NBSP " ")))
+
+(defun flatten-token-for-errormsg (x)
+  (cond ((opentok-p x)
+         (str::cat "<" (opentok-name x)
+                   (if (opentok-atts x) " [...]>" ">")))
+        ((closetok-p x)
+         (str::cat "</" (closetok-name x) ">"))
+        ((entitytok-p x)
+         (entitytok-as-entity x))
+        ((texttok-p x)
+         (texttok-text x))
+        (t
+         (er hard? 'flatten-token-for-errormsg "Invalid token ~x0" x))))
+
+(defun flatten-tokens-for-errormsg (x)
+  (if (atom x)
+      ""
+    (str::cat (flatten-token-for-errormsg (car x))
+              (flatten-tokens-for-errormsg (cdr x)))))
+
+(defun find-tag-imbalance (x open-tags loc)
+  "Returns (MV ERROR/NIL LOC/NIL)"
+  (b* (((when (atom x))
+        (mv (if open-tags
+                (str::cat (opentok-name (car open-tags)) " tag is never closed.")
+              nil)
+            nil))
+       ((when (opentok-p (car x)))
+        (find-tag-imbalance (cdr x) (cons (car x) open-tags) (+ 1 loc)))
+       ((when (closetok-p (car x)))
+        (b* ((close-name (closetok-name (car x)))
+             ((unless (consp open-tags))
+              (mv (str::cat "Found </" close-name "> with no matching opening tag.")
+                  loc))
+             (open-name (opentok-name (car open-tags)))
+             ((unless (equal close-name open-name))
+              (mv (str::cat "Found <" open-name "> with mismatched </" close-name ">.")
+                  loc)))
+          (find-tag-imbalance (cdr x) (cdr open-tags) (+ 1 loc)))))
+    (find-tag-imbalance (cdr x) open-tags (+ 1 loc))))
+
+(defun parse-xml (x)
+  (declare (type string x))
+  (b* (((mv err rtokens) (parse-xml-aux x 0 (length x) nil))
+       ((when err)
+        (mv err nil))
+       (tokens (reverse rtokens))
+       ((mv err loc) (find-tag-imbalance tokens nil 0))
+       ((when err)
+        (b* (((when (not loc))
+              (mv err nil))
+             (back-one (max 0 (- loc 2)))
+             (context  (take 4 (nthcdr back-one tokens)))
+             (nearby   (flatten-tokens-for-errormsg context)))
+          (mv (str::cat err "
+Nearby text: {" nearby "}" *nls*)
+              nil))))
+    (mv err tokens)))
