books/xdoc/preprocess.lisp
@@ -1,0 +1,883 @@
+; XDOC Documentation System for ACL2
+; Copyright (C) 2009-2010 Centaur Technology
+;
+; Contact:
+;   Centaur Technology Formal Verification Group
+;   7600-C N. Capital of Texas Highway, Suite 300, Austin, TX 78731, USA.
+;   http://www.centtech.com/
+;
+; This program is free software; you can redistribute it and/or modify it under
+; the terms of the GNU General Public License as published by the Free Software
+; Foundation; either version 2 of the License, or (at your option) any later
+; version.  This program is distributed in the hope that it will be useful but
+; WITHOUT ANY WARRANTY; without even the implied warranty of MERCHANTABILITY or
+; FITNESS FOR A PARTICULAR PURPOSE.  See the GNU General Public License for
+; more details.  You should have received a copy of the GNU General Public
+; License along with this program; if not, write to the Free Software
+; Foundation, Inc., 51 Franklin Street, Suite 500, Boston, MA 02110-1335, USA.
+;
+; Original author: Jared Davis <jared@centtech.com>
+
+
+; preprocess.lisp  -- the xdoc preprocessor
+
+(in-package "XDOC")
+(include-book "names")
+(include-book "str/top" :dir :system)
+(include-book "unicode/read-file-characters" :dir :system)
+(set-state-ok t)
+(program)
+
+
+(defun fmt-to-chars (string alist state) ;; ==> (MV CHARS STATE)
+
+; We can't use fmt to print directly to a string, which sucks.  So, we print to
+; a temporary file and read it back in.  This is truly horrible, but it's a lot
+; easier than reimplementing ppr.
+
+  (b* (((mv channel state)  (open-output-channel ".fmt-to-chars.tmp" :character state))
+       ((mv & state)        (fmt string alist channel state nil))
+       (state               (close-output-channel channel state))
+       ((mv data state)     (acl2::read-file-characters ".fmt-to-chars.tmp" state)))
+      (if (stringp data)
+          (prog2$
+           (cw "; xdoc note: in fmt-to-chars, failed to read .fmt-to-chars.tmp~%")
+           ;; In this funny return value, we insert a newline to be consistent
+           ;; with fmt.
+           (mv (coerce "
+[[ error reading .fmt-to-chars.tmp ]]" 'list)
+               state))
+        (mv data state))))
+
+
+(defun fmt-to-chars-and-encode (string alist state acc) ;; ==> (MV ACC-PRIME STATE)
+
+; Like fmt, but HTML-escape the result and accumulate it onto acc (in reverse
+; order) instead of printing it.
+
+  (mv-let (data state)
+          (fmt-to-chars string alist state)
+          ;; We cdr the data because fmt puts in a newline.
+          (let ((acc (simple-html-encode-chars (cdr data) acc)))
+            (mv acc state))))
+
+
+
+
+
+; ----------------- World Lookup Stuff --------------------------
+
+(defun get-formals (fn world)
+  (let ((formals (getprop fn 'formals :bad 'current-acl2-world world)))
+    (if (not (eq formals :bad))
+        formals
+      (let ((macro-args (getprop fn 'macro-args :bad 'current-acl2-world world)))
+        (if (not (eq macro-args :bad))
+            macro-args
+          (prog2$
+           (cw "; xdoc note: get-formals failed for ~s0::~s1.~%"
+               (symbol-package-name fn) (symbol-name fn))
+           (concatenate 'string
+                        "Error getting formals for "
+                        (symbol-package-name fn)
+                        "::"
+                        (symbol-name fn))))))))
+
+(defun get-measure (fn world)
+  (let ((just (getprop fn 'justification nil 'current-acl2-world world)))
+    (if just
+        (access justification just :measure)
+      (or (cw "; xdoc note: get-measure failed for ~x0.~%" fn)
+          (concatenate 'string
+                       "Error getting measure for "
+                       (symbol-package-name fn)
+                       "::"
+                       (symbol-name fn))))))
+
+(defun get-guard (fn world)
+  (if (not (eq (getprop fn 'formals :bad 'current-acl2-world world) :bad))
+      (getprop fn 'guard nil 'current-acl2-world world)
+    (prog2$
+     (cw "; xdoc note: get-guard failed for ~x0.~%" fn)
+     (concatenate 'string
+                  "Error getting guard for "
+                  (symbol-package-name fn)
+                  "::"
+                  (symbol-name fn)))))
+
+(defun get-body (fn world)
+  ;; This gets the original body normalized or non-normalized body based on
+  ;; what the user typed for the :normalize xarg.  The use of "last" skips past
+  ;; any other :definition rules that have been added since then.
+  (let ((bodies (getprop fn 'def-bodies nil 'current-acl2-world world)))
+    (if bodies
+        (access def-body (car (last bodies)) :concl)
+      (or (cw "; xdoc note: get-body failed for ~x0.~%" fn)
+          (concatenate 'string
+                       "Error getting body for "
+                       (symbol-package-name fn)
+                       "::"
+                       (symbol-name fn))))))
+
+(defun get-event (name world)
+  ;; A general purpose event lookup as in :pe
+  (let ((evt (acl2::get-event name world)))
+    (or evt
+        (cw "; xdoc note: get-event failed for ~x0.~%" name)
+        (concatenate 'string
+                     "Error getting event for "
+                     (symbol-package-name name)
+                     "::"
+                     (symbol-name name)))))
+
+(defun get-def (fn world)
+  ;; This used to do something else.  Now we try to be permissive.
+  (let ((def (acl2::get-def fn world)))
+    (if def
+        (cons 'defun def)
+      (get-event fn world))))
+
+(defun get-theorem (name world)
+  ;; BOZO maybe do some cleaning to remove hints, etc.
+  (get-event name world))
+
+
+;; (get-event 'append (w state))
+;; (get-def 'append (w state))
+;; (get-event 'binary-append (w state))
+;; (get-def 'binary-append (w state))
+;; (get-formals 'binary-append (w state))  ;; --> (ACL2::X ACL2::Y)
+;; (get-formals 'append (w state)) ;; --> (ACL2::X ACL2::Y &REST ACL2::RST)
+;; (get-measure 'binary-append (w state))
+;; (get-guard 'binary-append (w state))
+;; (get-body 'binary-append (w state))
+;; (get-def 'binary-append (w state))
+;; (get-theorem 'acl2::car-cons (w state))
+
+
+
+
+
+
+
+
+; -------------- Preprocessor Command Parsing  ------------------
+
+; Throughout these functions, X is a string we are traversing, N is our current
+; position in the string, XL is the length of the string, and an imagined guard
+; is:
+;
+;  (declare (xargs :guard (and (stringp x)
+;                              (natp n)
+;                              (natp xl)
+;                              (= xl (length x))
+;                              (<= n xl)))
+;
+; We could do a lot of this in logic mode, but there doesn't seem to be much
+; point to that.
+
+(defun error-context (x n xl) ;; ==> STRING
+  ;; Tries to show what text is near an error.
+  (declare (type string x))
+  (let ((min (nfix (- n 20)))
+        (max (min (+ n 20) xl)))
+    (subseq x min max)))
+
+; What a pain.  We have to implement a symbol parser.
+
+(defun parse-symbol-name-part (x n xl bar-escape-p slash-escape-p some-chars-p acc)
+  ;; ==> (MV ERROR NAME N-PRIME)
+  (declare (type string x))
+
+; This tries to read just one part of a symbol name (i.e., the package part,
+; or the name part.)
+
+  (if (= xl n)
+
+      ; End of string?  Error if we were escaped, or if we have not actually read
+      ; some characters yet.  Otherwise, it was okay.
+
+      (let ((result (reverse (coerce acc 'string))))
+        (if (or bar-escape-p slash-escape-p (not some-chars-p))
+            (mv (concatenate 'string "Near " (error-context x n xl)
+                             ": unexpected end of string while reading symbol.  "
+                             "Characters read so far: " result)
+                result n)
+          (mv nil result n)))
+
+    (let ((n+1  (+ n 1))
+          (char (char x n)))
+      (cond (slash-escape-p
+             ;; Slash escape is on, so just add next char verbatim and turn off
+             ;; slash escape.
+             (parse-symbol-name-part x n+1 xl bar-escape-p nil t (cons char acc)))
+            ((eql char #\|)
+             ;; Bar just toggles bar-escaped-ness.
+             (parse-symbol-name-part x n+1 xl (not bar-escape-p) nil t acc))
+            ((eql char #\\)
+             ;; Slash starts a slash-escape.
+             (parse-symbol-name-part x n+1 xl bar-escape-p t t acc))
+            (bar-escape-p
+             ;; Bar-escape is on and not a special char.  Read verbatim through it's
+             ;; turned off.
+             (parse-symbol-name-part x n+1 xl t nil t (cons char acc)))
+            ((member char '(#\Space #\( #\) #\Newline #\Tab #\Page #\: #\, #\' #\`))
+             ;; Whitespace, paren, colon, comma, quote, backquote, outside of a
+             ;; bar escape; end of symbol.  We can stop as long as we've actually
+             ;; read some characters.
+             (if some-chars-p
+                 (mv nil (reverse (coerce acc 'string)) n)
+               (mv (concatenate 'string "Near " (error-context x n xl) ": expected to read "
+                                "some part of a symbol, but found " (coerce (list char) 'string) ".")
+                   "" n)))
+            ((or (and (char<= #\a char) (char<= char #\z)))
+             ;; lowercase letters outside of bar escape get capitalized
+             (parse-symbol-name-part x n+1 xl nil nil t (cons (char-upcase char) acc)))
+            (t
+             ;; Otherwise add the char verbatim
+             (parse-symbol-name-part x n+1 xl nil nil t (cons char acc)))))))
+
+(defun parse-symbol (x n xl base-pkg) ;; ==> (MV ERROR SYMBOL N-PRIME)
+  (declare (type string x))
+
+; This extends parse-symbol-name-part to read both parts.  We support keywords,
+; etc.  This is definitely not going to handle everything in Common Lisp, but
+; whatever.
+
+  (if (= xl n)
+      (mv (concatenate 'string "Near " (error-context x n xl) ": end of string while "
+                       "trying to parse a symbol.")
+          nil n)
+    (let ((char (char x n)))
+      (if (eql char #\:)
+          ;; Starts with a colon.  Maybe it's keyword symbol?
+          (b* (((mv error name n)
+                (parse-symbol-name-part x (+ n 1) xl nil nil nil nil)))
+              (if error
+                  (mv error nil n)
+                (mv nil (intern-in-package-of-symbol name :keyword) n)))
+
+        ;; Doesn't start with a colon.
+        (b* (((mv error part1 n)
+              (parse-symbol-name-part x n xl nil nil nil nil))
+             ((when error)
+              (mv error nil n)))
+
+            (if (and (< (+ n 1) xl)
+                     (eql (char x n) #\:)
+                     (eql (char x (+ n 1)) #\:))
+                ;; "::" is matched.
+                (b* (((mv error part2 n)
+                      (parse-symbol-name-part x (+ n 2) xl nil nil nil nil))
+                     ((when error)
+                      (mv error nil n)))
+                    ;; Things look pretty good here.  One weird thing we will try
+                    ;; to detect is if there are extra colons, e.g.,
+                    ;; foo::bar::baz should be disallowed.  We really want a
+                    ;; whitespace or paren or quote or something
+                    (if (eql (char x n) #\:)
+                        (mv (concatenate 'string "Near " (error-context x n xl)
+                                         ": Three layers of colons in symbol name?")
+                            nil n)
+                      (mv nil (intern$ part2 part1) n)))
+
+              ;; Didn't match ::.
+              (if (and (< n xl)
+                       (eql (char x n) #\:))
+                  (mv (concatenate 'string "Near " (error-context x n xl)
+                                   ": Lone colon after symbol name?")
+                      nil n)
+
+                ;; We seem to have an okay package name, but no ::, so put
+                ;; it into the base package.
+                (mv nil (intern-in-package-of-symbol part1 base-pkg) n))))))))
+
+;; (defun test (x)
+;;   (declare (xargs :mode :program))
+;;   (parse-symbol x 0 (length x) 'acl2::foo))
+
+;; (test "foo")
+;; (test "bar")
+;; (test "123")
+;; (test "xdoc::bar)")
+;; (test "xdoc::|foo|)")
+;; (test "xdoc::bar12 ")
+;; (test ":foo)")
+;; (test ":|foo|)")
+;; (test ":")
+;; (test ":||")
+;; (test "||:")
+;; (test "::|foo|)")
+;; (test "acl2:::bar)")
+;; (test "acl2::bar)")
+;; (test "acl2::bar:")
+;; (test "acl2::bar|:|)")
+
+(defun read-literal (x n xl chars) ;; ==> (MV SUCCESSP N-PRIME)
+  ;; Try to read CHARS, verbatim.
+  (declare (type string x))
+  (cond ((= n xl)
+         (mv (atom chars) n))
+        ((consp chars)
+         (if (eql (char x n) (car chars))
+             (read-literal x (+ n 1) xl (cdr chars))
+           (mv nil n)))
+        (t
+         (mv t n))))
+
+(defun read-through-some-char-aux (x n xl chars acc) ;; ==> (MV SUCCESSP STRING N-PRIME)
+  (declare (type string x))
+  (if (= xl n)
+      (mv nil (reverse (coerce acc 'string)) n)
+    (let ((charN (char x n)))
+      (if (member charN chars)
+          (mv t (reverse (coerce (cons charN acc) 'string)) n)
+        (read-through-some-char-aux x (+ 1 n) xl chars (cons charN acc))))))
+
+(defun read-through-some-char (x n xl chars)
+  ;; Try to read until one of CHARS is found
+  (declare (type string x))
+  (read-through-some-char-aux x n xl chars nil))
+
+(defun skip-past-ws (x n xl) ;; ==> N-PRIME
+  (declare (type string x))
+  (cond ((= xl n)
+         n)
+        ((member (char x n) '(#\Space #\Tab #\Newline #\Page))
+         (skip-past-ws x (+ 1 n) xl))
+        (t
+         n)))
+
+(defun parse-directive (x n xl base-pkg) ;; ==> (MV ERROR COMMAND ARG N-PRIME)
+  ;; Every directive has the form @(command arg)
+  ;; Where command and arg are symbols.
+  ;; We assume @( has just been read, and N is now pointing right after the open paren.
+  (declare (type string x))
+  (b* ((n                    (skip-past-ws x n xl))
+       ((mv error command n) (parse-symbol x n xl (pkg-witness "XDOC")))
+       ((when error)
+        (mv error nil nil n))
+       (n                    (skip-past-ws x n xl))
+       ((mv error arg n)     (parse-symbol x n xl base-pkg)))
+      (cond
+       ;; Some error parsing arg.  Add a little more context.
+       (error (mv (concatenate 'string "In " (symbol-name command) " directive: " error)
+                  nil nil n))
+
+       ;; Ends with ), good.
+       ((and (< n xl)
+             (eql (char x n) #\)))
+        (mv nil command arg (+ n 1)))
+
+       (t
+        (mv (concatenate 'string "In " (symbol-name command) " directive, expected ) after "
+                         (symbol-name arg)
+                         ". Near " (error-context x n xl) ".")
+            nil nil n)))))
+
+;; (let ((x "body foo)"))
+;;   (parse-directive x 0 (length x) 'acl2::foo))
+
+;; (let ((x "body foo) bar"))
+;;   (parse-directive x 0 (length x) 'acl2::foo))
+
+;; (let ((x "body xdoc::foo) bar"))
+;;   (parse-directive x 0 (length x) 'acl2::foo))
+
+;; (let ((x "xdoc::body xdoc::foo) bar"))
+;;   (parse-directive x 0 (length x) 'acl2::foo))
+
+;; (let ((x "acl2::body xdoc::foo) bar"))
+;;   (parse-directive x 0 (length x) 'acl2::foo))
+
+;; (let ((x "acl2::body)xdoc::foo) bar"))
+;;   (parse-directive x 0 (length x) 'acl2::foo))
+
+
+
+
+; -------------- Executing Directives ---------------------------
+
+(defun process-url-directive (arg state acc) ;; ===> (MV ACC STATE)
+
+; @(url foo) just expands into the file name for foo.
+
+  (b* ((acc            (file-name-mangle arg acc)))
+      (mv acc state)))
+
+
+(defun process-sym-directive (arg base-pkg state acc) ;; ===> (MV ACC STATE)
+
+; @(sym foo) just expands into the standard name mangling for foo
+
+  (b* ((acc            (sym-mangle arg base-pkg acc)))
+      (mv acc state)))
+
+
+(defun process-sym-cap-directive (arg base-pkg state acc) ;; ===> (MV ACC STATE)
+
+; @(csym foo) just expands into the standard capitalized name mangling for foo
+
+  (b* ((acc            (sym-mangle-cap arg base-pkg acc)))
+      (mv acc state)))
+
+
+(defun process-see-directive (arg base-pkg state acc) ;; ===> (MV ACC STATE)
+
+; @(see foo) just expands into a link with a lowercase name.
+
+  (b* ((acc            (str::revappend-chars "<see topic=\"" acc))
+       (acc            (file-name-mangle arg acc))
+       (acc            (str::revappend-chars "\">" acc))
+       (acc            (sym-mangle arg base-pkg acc))
+       (acc            (str::revappend-chars "</see>" acc)))
+      (mv acc state)))
+
+
+(defun process-see-cap-directive (arg base-pkg state acc) ;; ===> (MV ACC STATE)
+
+; @(csee foo) just expands into a link with a capitalized name.
+
+  (b* ((acc            (str::revappend-chars "<see topic=\"" acc))
+       (acc            (file-name-mangle arg acc))
+       (acc            (str::revappend-chars "\">" acc))
+       (acc            (sym-mangle-cap arg base-pkg acc))
+       (acc            (str::revappend-chars "</see>" acc)))
+      (mv acc state)))
+
+
+(defconst *xdoc-link-file-message*
+  "; This is an XDOC Link file.
+; Ordinarily, you should not see this file.
+;
+; If you are viewing this file in a web browser, you probably
+; have not configured your web browser to send .xdoc-link files
+; to Emacs.
+;
+;   (Or, if you have already done that, but you accessed this
+;    file through a web server, the server may just not be
+;    assigning .xdoc-link files the appropriate MIME type.)
+;
+; If you are viewing this file in Emacs, you probably have not
+; loaded xdoc.el from the xdoc/ directory.
+;
+; Please see the XDOC manual for more information.")
+
+(defun process-srclink-directive (arg dir state acc) ;; ===> (MV ACC STATE)
+
+; We do two things:
+;
+;   1. Extend acc with a srclink tag, and
+;
+;   2. Write a .xdoc-link file to dir for this tag, unless DIR is NIL in
+;      which case we skip this step
+;
+; This is kind of ugly in that we may write the same .xdoc-link file many
+; times, but this doesn't seem to practically be a problem.
+;
+; Our emacs linking mechanism is slightly broken, in that all we can tell emacs
+; is the name of a symbol to look for using its tags mechanism.  We are hoping
+; that:
+;
+;   1. The user has the appropriate TAGS tables set up (reasonable),
+;
+;   2. The symbol is actually defined in a source file somewhere, instead of
+;      being introduced by a macro or something, and
+;
+;   3. The symbol is not defined in multiple packages, so that the user will be
+;      taken to the right source file.  (That is, we can't tell emacs something
+;      like "foo::bar", because it doesn't understand (in-package ...); We can
+;      only tell it to search for bar.)
+;
+; Whether or not #2 and #3 hold is a total crap-shoot, and we're basically
+; hoping that most of the time find-tag will take them to the right place.
+
+  (b* ((shortname (coerce (string-downcase (symbol-name arg)) 'list))
+       (filename  (concatenate 'string
+                               (reverse (coerce (file-name-mangle arg nil) 'string))
+                               ".xdoc-link"))
+
+       (acc (str::revappend-chars "<srclink file=\"" acc))
+       (acc (str::revappend-chars filename acc))
+       (acc (str::revappend-chars "\">" acc))
+       (acc (simple-html-encode-chars shortname acc))
+       (acc (str::revappend-chars "</srclink>" acc))
+
+       ((unless dir)
+        (mv acc state))
+
+       (fullpath           (acl2::extend-pathname dir filename state))
+       ((mv channel state) (open-output-channel fullpath :character state))
+       (state (princ$ *xdoc-link-file-message* channel state))
+       (state (newline channel state))
+       (state (newline channel state))
+       (state (princ$ (coerce shortname 'string) channel state))
+       (state (newline channel state))
+       (state (close-output-channel channel state)))
+      (mv acc state)))
+
+(defun process-body-directive (arg state acc) ;; ===> (MV ACC STATE)
+
+; @(body foo) -- look up the body and pretty-print it in a <code> block.
+
+  (b* ((body           (get-body arg (w state)))
+       (acc            (str::revappend-chars "<code>" acc))
+       ((mv acc state) (fmt-to-chars-and-encode "~x0"
+                                                (list (cons #\0 body))
+                                                state acc))
+       (acc            (str::revappend-chars "</code>" acc)))
+      (mv acc state)))
+
+(defun process-def-directive (arg dir state acc) ;; ===> (MV ACC STATE)
+
+; @(def foo) -- look up the definition for foo, pretty-print it in a <code>
+; block, along with a source-code link.
+
+  (b* ((def            (get-def arg (w state)))
+       (acc            (str::revappend-chars "<p><b>Definition: </b>" acc))
+       ((mv acc state) (process-srclink-directive arg dir state acc))
+       (acc            (str::revappend-chars "</p>" acc))
+       (acc            (str::revappend-chars "<code>" acc))
+       ((mv acc state) (fmt-to-chars-and-encode "~x0"
+                                                (list (cons #\0 def))
+                                                state acc))
+       (acc            (str::revappend-chars "</code>" acc)))
+      (mv acc state)))
+
+(defun process-gdef-directive (arg base-pkg state acc) ;; ===> (MV ACC STATE)
+
+; @(gdef foo) -- Look up the definition for foo, pretty-print it as in @def,
+; but don't use a source-code link because this is a "Generated Definition" for
+; which a tags-search will probably fail.
+
+  (b* ((def            (get-def arg (w state)))
+       (acc            (str::revappend-chars "<p><b>Definition: </b>" acc))
+       (acc            (sym-mangle arg base-pkg acc))
+       (acc            (str::revappend-chars "</p>" acc))
+       (acc            (str::revappend-chars "<code>" acc))
+       ((mv acc state) (fmt-to-chars-and-encode "~x0"
+                                                (list (cons #\0 def))
+                                                state acc))
+       (acc            (str::revappend-chars "</code>" acc)))
+      (mv acc state)))
+
+(defun process-thm-directive (arg dir state acc) ;; ===> (MV ACC STATE)
+
+; @(thm foo) -- Look up the theorem named foo, and pretty-print its event along
+; with a source link.
+
+  (b* ((theorem        (get-theorem arg (w state)))
+       (acc            (str::revappend-chars "<p><b>Theorem: </b>" acc))
+       ((mv acc state) (process-srclink-directive arg dir state acc))
+       (acc            (str::revappend-chars "</p>" acc))
+       (acc            (str::revappend-chars "<code>" acc))
+       ((mv acc state) (fmt-to-chars-and-encode "~x0"
+                                                (list (cons #\0 theorem))
+                                                state acc))
+       (acc            (str::revappend-chars "</code>" acc)))
+      (mv acc state)))
+
+(defun process-gthm-directive (arg base-pkg state acc) ;; ===> (MV ACC STATE)
+
+; @(gthm foo) -- Like @(thm foo), but don't provide a source link since this is
+; a generated theorem.
+
+  (b* ((theorem        (get-theorem arg (w state)))
+       (acc            (str::revappend-chars "<p><b>Theorem: </b>" acc))
+       (acc            (sym-mangle arg base-pkg acc))
+       (acc            (str::revappend-chars "</p>" acc))
+       (acc            (str::revappend-chars "<code>" acc))
+       ((mv acc state) (fmt-to-chars-and-encode "~x0"
+                                                (list (cons #\0 theorem))
+                                                state acc))
+       (acc            (str::revappend-chars "</code>" acc)))
+      (mv acc state)))
+
+(defun process-formals-directive (arg state acc) ;; ===> (MV ACC STATE)
+
+; @(formals foo) -- just find the formals for foo and print them without any
+; extra formatting.
+
+  (b* ((formals        (get-formals arg (w state)))
+       ((mv acc state) (fmt-to-chars-and-encode "~x0"
+                                                (list (cons #\0 formals))
+                                                state acc)))
+      (mv acc state)))
+
+(defun process-call-directive (arg state acc) ;; ===> (MV ACC STATE)
+
+; @(call foo) -- find the formals to foo and insert <tt>(foo x y z)</tt>.
+; BOZO consider adding an emacs link.
+
+  (b* ((formals        (get-formals arg (w state)))
+       (call           (cons arg formals))
+       (acc            (str::revappend-chars "<tt>" acc))
+       ((mv acc state) (fmt-to-chars-and-encode "~x0"
+                                                (list (cons #\0 call))
+                                                state acc))
+       (acc            (str::revappend-chars "</tt>" acc)))
+      (mv acc state)))
+
+(defun process-ccall-directive (arg state acc) ;; ===> (MV ACC STATE)
+
+; @(ccall foo) -- "code call" is like @(call foo), but uses <code> instead
+; of <tt> tags.
+
+  (b* ((formals        (get-formals arg (w state)))
+       (call           (cons arg formals))
+       (acc            (str::revappend-chars "<code>" acc))
+       ((mv acc state) (fmt-to-chars-and-encode "~x0"
+                                                (list (cons #\0 call))
+                                                state acc))
+       (acc            (str::revappend-chars "</code>" acc)))
+      (mv acc state)))
+
+(defun process-measure-directive (arg state acc) ;; ===> (MV ACC STATE)
+
+; @(measure foo) -- find the measure for foo and print it without any extra
+; formatting.
+
+  (b* ((measure        (get-measure arg (w state)))
+       ((mv acc state) (fmt-to-chars-and-encode "~x0"
+                                                (list (cons #\0 measure))
+                                                state acc)))
+      (mv acc state)))
+
+
+(defun process-directive (command arg dir base-pkg state acc) ;; ===> (MV ACC STATE)
+
+; Command and Arg are the already-parsed symbols we have read from the
+; documentation string.  Carry out whatever directive we've been asked to do.
+; DIR is the output dir.  Acc is the accumulator for our output characters.
+
+  (case command
+    (def       (process-def-directive arg dir state acc))
+    (thm       (process-thm-directive arg dir state acc))
+    (srclink   (process-srclink-directive arg dir state acc))
+    (gdef      (process-gdef-directive arg base-pkg state acc))
+    (gthm      (process-gthm-directive arg base-pkg state acc))
+    (body      (process-body-directive arg state acc))
+    (formals   (process-formals-directive arg state acc))
+    (measure   (process-measure-directive arg state acc))
+    (call      (process-call-directive arg state acc))
+    (ccall     (process-ccall-directive arg state acc))
+    (url       (process-url-directive arg state acc))
+    (see       (process-see-directive arg base-pkg state acc))
+    (csee      (process-see-cap-directive arg base-pkg state acc))
+    (sym       (process-sym-directive arg base-pkg state acc))
+    (csym      (process-sym-cap-directive arg base-pkg state acc))
+    (otherwise
+     (prog2$
+      (cw "; xdoc error: unknown directive ~x0.~%" command)
+      (let* ((acc (str::revappend-chars "[[ unknown directive " acc))
+             (acc (str::revappend-chars (symbol-package-name command) acc))
+             (acc (str::revappend-chars "::" acc))
+             (acc (str::revappend-chars (symbol-name command) acc))
+             (acc (str::revappend-chars "]]" acc)))
+        (mv acc state))))))
+
+
+
+
+; Ugly special hacks for some problems with <code> segments.
+;
+; As an example, consider:
+;
+;  |(defxdoc ...
+;  |  :long "<p>blah blah blah</p>
+;  |
+;  |<p>blah blah blah</p>
+;  |
+;  |<code>
+;  |(example-sexpr ...)
+;  |</code>
+;  |
+;  |<p>blah blah blah</p>")
+;
+; The <code> block above causes problems for Emacs, because the algorithm for
+; figuring out where an S-expression begins seems to basically look for an
+; opening paren at the start of a line.  The result is that Emacs thinks the
+; "(example-sexpr ...)" is the start of a form, rather than the "(defxdoc
+; ...)," which can cause incorrect and irritating syntax highlighting, and can
+; also cause problems for commands like "C-t e" that want to send a form to the
+; *shell* buffer.  To cope with this, I typically indent <code> blocks with a
+; single space, e.g.,
+;
+;  |<code>                   instead of    |<code>
+;  | (example-sexpr ...)                   |(example-sexpr ...)
+;  |</code>                                |</code>
+;
+; but, this convention isn't followed by the code blocks introduced with @(def
+; ...)  and similar, and so the <code> blocks I write may not line up right
+; with generated code blocks.
+;
+; To fix this, we look at the text between <code> and </code>, and if every
+; line begins with a space, we eat those spaces.
+
+(encapsulate
+  ()
+  (local (defthm first-n-ac-expand
+           (implies (syntaxp (quotep i))
+                    (equal (first-n-ac i l ac)
+                           (cond ((zp i) (reverse ac))
+                                 (t (first-n-ac (1- i)
+                                                (cdr l)
+                                                (cons (car l) ac))))))))
+
+  (defun just-started-code-p (acc)
+    (declare (xargs :guard (true-listp acc)))
+    (mbe :logic (equal (take 6 acc)
+                       (reverse (coerce "<code>" 'list)))
+         :exec
+         (and (consp (cdr (cdr (cdr (cdr (cdr acc))))))
+              (eql (first acc) #\>)
+              (eql (second acc) #\e)
+              (eql (third acc) #\d)
+              (eql (fourth acc) #\o)
+              (eql (fifth acc) #\c)
+              (eql (sixth acc) #\<)))))
+
+(defun read-code-segment (x n xl acc always-spacep)
+  "Returns (MV N ACC ALWAYS-SPACEP)"
+
+; We assume we're inside a <code> block.  We read until a < character is
+; encountered, gathering the characters we see and tracking whether each
+; newline is followed by a space.
+
+  (b* (((when (>= n xl))
+        (mv n acc always-spacep))
+
+       (char-n (char x n))
+       ((when (eql char-n #\<))
+        ;; We assume this is the </code> tag and stop reading.
+        (mv n acc always-spacep))
+
+       (acc (cons char-n acc))
+       ((unless (eql char-n #\Newline))
+        ;; A normal character, just accumulate it.
+        (read-code-segment x (+ 1 n) xl acc always-spacep))
+
+       (n (+ 1 n))
+       ((when (>= n xl))
+        ;; End of string while reading <code>?  Shouldn't really happen...
+        (mv n acc always-spacep))
+
+       (char-n (char x n))
+       ((when (eql char-n #\<))
+        ;; We allow the </code> to come without a space.
+        (mv n acc always-spacep))
+
+       (acc (cons char-n acc))
+       (always-spacep (and always-spacep
+                           (or (eql char-n #\Space)
+                               (eql char-n #\Newline)))))
+    (read-code-segment x (+ 1 n) xl acc always-spacep)))
+
+(defun revappend-code-chars (code-chars acc always-spacep)
+  (b* (((when (atom code-chars))
+        acc)
+       (char1 (car code-chars))
+       (acc   (cons char1 acc))
+       ((unless (eql char1 #\Newline))
+        (revappend-code-chars (cdr code-chars) acc always-spacep))
+       ((when (and always-spacep
+                   (consp (cdr code-chars))
+                   (eql (second code-chars) #\Space)))
+        ;; Skip the first space
+        (revappend-code-chars (cddr code-chars) acc always-spacep)))
+    (revappend-code-chars (cdr code-chars) acc always-spacep)))
+
+(defun transform-code-segments (x n xl acc)
+  (b* (((when (>= n xl))
+        acc)
+       (char-n (char x n))
+       (acc    (cons char-n acc))
+       (n      (+ 1 n))
+       ((unless (and (eql char-n #\>)
+                     (just-started-code-p acc)))
+        (transform-code-segments x n xl acc))
+       ;; Started a code segment.
+       ((mv n code-acc always-spacep)
+        (read-code-segment x n xl nil t))
+       (code-chars (reverse code-acc))
+       (acc (revappend-code-chars code-chars acc always-spacep)))
+    (transform-code-segments x n xl acc)))
+
+(defun transform-code (x)
+  ;; Fix leading spaces in <code> segments
+  (reverse (coerce (transform-code-segments x 0 (length x) nil) 'string)))
+
+;; (transform-code 
+;; "<p>This is 
+;; some regular text</p>
+;; <code>
+;;   blah1
+;; blah2
+;;   blah3
+;; </code>
+;; <p>And more text</p>")
+
+(defun preprocess-aux (x n xl dir base-pkg state acc)
+  "Returns (MV ACC STATE)"
+  (declare (type string x))
+
+; Main preprocessor loop.  Read from the string and accumulate the result into
+; acc, expanding away any preprocessor directives.
+
+  (b* (((when (= n xl))
+        (mv acc state))
+
+       (char (char x n))
+       ((when (eql char #\@))
+        (cond ((and (< (+ n 1) xl)
+                    (eql (char x (+ n 1)) #\@))
+               ;; @@ --> @
+               (preprocess-aux x (+ n 2) xl dir base-pkg state (cons #\@ acc)))
+
+              ((and (< (+ n 1) xl)
+                    (eql (char x (+ n 1)) #\())
+               ;; @( --> directive
+               (b* (((mv error command arg n) (parse-directive x (+ n 2) xl base-pkg))
+                    ((when error)
+                     (prog2$ (cw "; xdoc error: ~x0.~%" error)
+                             (mv acc state)))
+                    ((mv acc state)
+                     (process-directive command arg dir base-pkg state acc)))
+                 (preprocess-aux x n xl dir base-pkg state acc)))
+
+              (t
+               ;; @ sign in some other context.
+               (preprocess-aux x (+ n 1) xl dir base-pkg state (cons #\@ acc)))))
+
+       ((when (eql char #\Newline))
+        ;; Gross hack #1: eat initial newlines from the start of a <code>
+        ;; block, since otherwise they look ugly when firefox renders them.
+        (if (just-started-code-p acc)
+            (if (and (< (+ n 1) xl)
+                     (eql (char x (+ n 1)) #\Newline))
+                ;; Avoid eating multiple newlines at the start of a code block.
+                (preprocess-aux x (+ n 2) xl dir base-pkg state (cons #\Newline acc))
+              (preprocess-aux x (+ n 1) xl dir base-pkg state acc))
+          ;; Gross hack #2: the XSLT transformer in firefox seems to have some
+          ;; problems if there aren't spaces at the end of lines, e.g., it will
+          ;; run together the hover-text in the hierarchical description in
+          ;; preview.html.  Fix by putting a space before newlines.  Horrible.
+          (preprocess-aux x (+ n 1) xl dir base-pkg state (list* #\Newline #\Space acc)))))
+
+    ;; Otherwise just keep the char and keep going.
+    (preprocess-aux x (+ n 1) xl dir base-pkg state (cons char acc))))
+
+(defun preprocess-main (x dir base-pkg state acc)
+  (declare (type string x))
+  (b* ((current-pkg    (acl2::f-get-global 'current-package state))
+       ;; Temporarily make "fmt" print as if it's in base-pkg.
+       ((mv & & state) (acl2::set-current-package (symbol-package-name base-pkg) state))
+       (x              (transform-code x))
+       ((mv acc state) (preprocess-aux x 0 (length x) dir base-pkg state acc))
+       ;; Restore base-pkg for whoever called us.
+       ((mv & & state) (acl2::set-current-package current-pkg state)))
+      (mv acc state)))
+
+
+
+
