books/xdoc/save.lisp
@@ -18,22 +18,38 @@
 ;
 ; Original author: Jared Davis <jared@centtech.com>
 
-(in-package "XDOC")
-(include-book "defxdoc")
-(include-book "defxdoc-raw")
-(include-book "names")
-(include-book "str/top" :dir :system)
-(include-book "unicode/read-file-characters" :dir :system)
-(include-book "finite-set-theory/osets/sets" :dir :system)
-(set-state-ok t)
-(program)
-
-
 ; save.lisp
 ;
 ; This file defines the XDOC functions for running the preprocessor and saving
-; XML files.  Normally you should not include this file except in a script that
-; generates your manual.
+; XML files.  Note that the save-topics command we introduce cannot actually be
+; used unless the mkdir-raw book is loaded first.  This is automatically handled
+; by the "save" macro in top.lisp.
+
+(in-package "XDOC")
+(include-book "mkdir")
+(include-book "base")
+(include-book "preprocess")
+(include-book "parse-xml")
+(include-book "tools/progndollar" :dir :system)
+(include-book "finite-set-theory/osets/sets" :dir :system)
+(set-state-ok t)
+
+(defun cw-princ$ (str)
+  ;; Same as princ$ to *standard-co*, but doesn't require state.
+  (declare (xargs :guard t))
+  (mbe :logic nil
+       :exec
+       (wormhole 'cw-raw-wormhole
+                 '(lambda (whs) whs)
+                 nil
+                 `(let ((state (princ$ ',str *standard-co* state)))
+                    (value :q))
+                 :ld-prompt nil
+                 :ld-pre-eval-print nil
+                 :ld-post-eval-print nil
+                 :ld-verbose nil)))
+
+(program)
 
 
 ; --------------------- File Copying ----------------------------
@@ -68,695 +84,6 @@
          (destfile (acl2::extend-pathname destdir (car filenames) state))
          (state    (stupid-copy-file srcfile destfile state)))
         (stupid-copy-files srcdir (cdr filenames) destdir state))))
-
-
-
-; -------------  HTML encoding, IO help -------------------------
-
-(defun fmt-to-chars (string alist state) ;; ==> (MV CHARS STATE)
-
-; We can't use fmt to print directly to a string, which sucks.  So, we print to
-; a temporary file and read it back in.  This is truly horrible, but it's a lot
-; easier than reimplementing ppr.
-
-  (b* (((mv channel state)  (open-output-channel ".fmt-to-chars.tmp" :character state))
-       ((mv & state)        (fmt string alist channel state nil))
-       (state               (close-output-channel channel state))
-       ((mv data state)     (acl2::read-file-characters ".fmt-to-chars.tmp" state)))
-      (if (stringp data)
-          (prog2$
-           (cw "; xdoc note: in fmt-to-chars, failed to read .fmt-to-chars.tmp~%")
-           ;; In this funny return value, we insert a newline to be consistent
-           ;; with fmt.
-           (mv (coerce "
-[[ error reading .fmt-to-chars.tmp ]]" 'list)
-               state))
-        (mv data state))))
-
-
-(defun fmt-to-chars-and-encode (string alist state acc) ;; ==> (MV ACC-PRIME STATE)
-
-; Like fmt, but HTML-escape the result and accumulate it onto acc (in reverse
-; order) instead of printing it.
-
-  (mv-let (data state)
-          (fmt-to-chars string alist state)
-          ;; We cdr the data because fmt puts in a newline.
-          (let ((acc (simple-html-encode-chars (cdr data) acc)))
-            (mv acc state))))
-
-
-
-
-
-; ----------------- World Lookup Stuff --------------------------
-
-(defun get-formals (fn world)
-  (let ((formals (getprop fn 'formals :bad 'current-acl2-world world)))
-    (if (not (eq formals :bad))
-        formals
-      (let ((macro-args (getprop fn 'macro-args :bad 'current-acl2-world world)))
-        (if (not (eq macro-args :bad))
-            macro-args
-          (prog2$
-           (cw "; xdoc note: get-formals failed for ~s0::~s1.~%"
-               (symbol-package-name fn) (symbol-name fn))
-           (concatenate 'string
-                        "Error getting formals for "
-                        (symbol-package-name fn)
-                        "::"
-                        (symbol-name fn))))))))
-
-(defun get-measure (fn world)
-  (let ((just (getprop fn 'justification nil 'current-acl2-world world)))
-    (if just
-        (access justification just :measure)
-      (or (cw "; xdoc note: get-measure failed for ~x0.~%" fn)
-          (concatenate 'string
-                       "Error getting measure for "
-                       (symbol-package-name fn)
-                       "::"
-                       (symbol-name fn))))))
-
-(defun get-guard (fn world)
-  (if (not (eq (getprop fn 'formals :bad 'current-acl2-world world) :bad))
-      (getprop fn 'guard nil 'current-acl2-world world)
-    (prog2$
-     (cw "; xdoc note: get-guard failed for ~x0.~%" fn)
-     (concatenate 'string
-                  "Error getting guard for "
-                  (symbol-package-name fn)
-                  "::"
-                  (symbol-name fn)))))
-
-(defun get-body (fn world)
-  ;; This gets the original body normalized or non-normalized body based on
-  ;; what the user typed for the :normalize xarg.  The use of "last" skips past
-  ;; any other :definition rules that have been added since then.
-  (let ((bodies (getprop fn 'def-bodies nil 'current-acl2-world world)))
-    (if bodies
-        (access def-body (car (last bodies)) :concl)
-      (or (cw "; xdoc note: get-body failed for ~x0.~%" fn)
-          (concatenate 'string
-                       "Error getting body for "
-                       (symbol-package-name fn)
-                       "::"
-                       (symbol-name fn))))))
-
-(defun get-event (name world)
-  ;; A general purpose event lookup as in :pe
-  (let ((evt (acl2::get-event name world)))
-    (or evt
-        (cw "; xdoc note: get-event failed for ~x0.~%" name)
-        (concatenate 'string
-                     "Error getting event for "
-                     (symbol-package-name name)
-                     "::"
-                     (symbol-name name)))))
-
-(defun get-def (fn world)
-  ;; This used to do something else.  Now we try to be permissive.
-  (let ((def (acl2::get-def fn world)))
-    (if def
-        (cons 'defun def)
-      (get-event fn world))))
-
-(defun get-theorem (name world)
-  ;; BOZO maybe do some cleaning to remove hints, etc.
-  (get-event name world))
-
-
-;; (get-event 'append (w state))
-;; (get-def 'append (w state))
-;; (get-event 'binary-append (w state))
-;; (get-def 'binary-append (w state))
-;; (get-formals 'binary-append (w state))  ;; --> (ACL2::X ACL2::Y)
-;; (get-formals 'append (w state)) ;; --> (ACL2::X ACL2::Y &REST ACL2::RST)
-;; (get-measure 'binary-append (w state))
-;; (get-guard 'binary-append (w state))
-;; (get-body 'binary-append (w state))
-;; (get-def 'binary-append (w state))
-;; (get-theorem 'acl2::car-cons (w state))
-
-
-
-
-
-
-
-
-; -------------- Preprocessor Command Parsing  ------------------
-
-; Throughout these functions, X is a string we are traversing, N is our current
-; position in the string, XL is the length of the string, and an imagined guard
-; is:
-;
-;  (declare (xargs :guard (and (stringp x)
-;                              (natp n)
-;                              (natp xl)
-;                              (= xl (length x))
-;                              (<= n xl)))
-;
-; We could do a lot of this in logic mode, but there doesn't seem to be much
-; point to that.
-
-(defun error-context (x n xl) ;; ==> STRING
-  ;; Tries to show what text is near an error.
-  (declare (type string x))
-  (let ((min (nfix (- n 20)))
-        (max (min (+ n 20) xl)))
-    (subseq x min max)))
-
-; What a pain.  We have to implement a symbol parser.
-
-(defun parse-symbol-name-part (x n xl bar-escape-p slash-escape-p some-chars-p acc)
-  ;; ==> (MV ERROR NAME N-PRIME)
-  (declare (type string x))
-
-; This tries to read just one part of a symbol name (i.e., the package part,
-; or the name part.)
-
-  (if (= xl n)
-
-      ; End of string?  Error if we were escaped, or if we have not actually read
-      ; some characters yet.  Otherwise, it was okay.
-
-      (let ((result (reverse (coerce acc 'string))))
-        (if (or bar-escape-p slash-escape-p (not some-chars-p))
-            (mv (concatenate 'string "Near " (error-context x n xl)
-                             ": unexpected end of string while reading symbol.  "
-                             "Characters read so far: " result)
-                result n)
-          (mv nil result n)))
-
-    (let ((n+1  (+ n 1))
-          (char (char x n)))
-      (cond (slash-escape-p
-             ;; Slash escape is on, so just add next char verbatim and turn off
-             ;; slash escape.
-             (parse-symbol-name-part x n+1 xl bar-escape-p nil t (cons char acc)))
-            ((eql char #\|)
-             ;; Bar just toggles bar-escaped-ness.
-             (parse-symbol-name-part x n+1 xl (not bar-escape-p) nil t acc))
-            ((eql char #\\)
-             ;; Slash starts a slash-escape.
-             (parse-symbol-name-part x n+1 xl bar-escape-p t t acc))
-            (bar-escape-p
-             ;; Bar-escape is on and not a special char.  Read verbatim through it's
-             ;; turned off.
-             (parse-symbol-name-part x n+1 xl t nil t (cons char acc)))
-            ((member char '(#\Space #\( #\) #\Newline #\Tab #\Page #\: #\, #\' #\`))
-             ;; Whitespace, paren, colon, comma, quote, backquote, outside of a
-             ;; bar escape; end of symbol.  We can stop as long as we've actually
-             ;; read some characters.
-             (if some-chars-p
-                 (mv nil (reverse (coerce acc 'string)) n)
-               (mv (concatenate 'string "Near " (error-context x n xl) ": expected to read "
-                                "some part of a symbol, but found " (coerce (list char) 'string) ".")
-                   "" n)))
-            ((or (and (char<= #\a char) (char<= char #\z)))
-             ;; lowercase letters outside of bar escape get capitalized
-             (parse-symbol-name-part x n+1 xl nil nil t (cons (char-upcase char) acc)))
-            (t
-             ;; Otherwise add the char verbatim
-             (parse-symbol-name-part x n+1 xl nil nil t (cons char acc)))))))
-
-(defun parse-symbol (x n xl base-pkg) ;; ==> (MV ERROR SYMBOL N-PRIME)
-  (declare (type string x))
-
-; This extends parse-symbol-name-part to read both parts.  We support keywords,
-; etc.  This is definitely not going to handle everything in Common Lisp, but
-; whatever.
-
-  (if (= xl n)
-      (mv (concatenate 'string "Near " (error-context x n xl) ": end of string while "
-                       "trying to parse a symbol.")
-          nil n)
-    (let ((char (char x n)))
-      (if (eql char #\:)
-          ;; Starts with a colon.  Maybe it's keyword symbol?
-          (b* (((mv error name n)
-                (parse-symbol-name-part x (+ n 1) xl nil nil nil nil)))
-              (if error
-                  (mv error nil n)
-                (mv nil (intern-in-package-of-symbol name :keyword) n)))
-
-        ;; Doesn't start with a colon.
-        (b* (((mv error part1 n)
-              (parse-symbol-name-part x n xl nil nil nil nil))
-             ((when error)
-              (mv error nil n)))
-
-            (if (and (< (+ n 1) xl)
-                     (eql (char x n) #\:)
-                     (eql (char x (+ n 1)) #\:))
-                ;; "::" is matched.
-                (b* (((mv error part2 n)
-                      (parse-symbol-name-part x (+ n 2) xl nil nil nil nil))
-                     ((when error)
-                      (mv error nil n)))
-                    ;; Things look pretty good here.  One weird thing we will try
-                    ;; to detect is if there are extra colons, e.g.,
-                    ;; foo::bar::baz should be disallowed.  We really want a
-                    ;; whitespace or paren or quote or something
-                    (if (eql (char x n) #\:)
-                        (mv (concatenate 'string "Near " (error-context x n xl)
-                                         ": Three layers of colons in symbol name?")
-                            nil n)
-                      (mv nil (intern$ part2 part1) n)))
-
-              ;; Didn't match ::.
-              (if (and (< n xl)
-                       (eql (char x n) #\:))
-                  (mv (concatenate 'string "Near " (error-context x n xl)
-                                   ": Lone colon after symbol name?")
-                      nil n)
-
-                ;; We seem to have an okay package name, but no ::, so put
-                ;; it into the base package.
-                (mv nil (intern-in-package-of-symbol part1 base-pkg) n))))))))
-
-;; (defun test (x)
-;;   (declare (xargs :mode :program))
-;;   (parse-symbol x 0 (length x) 'acl2::foo))
-
-;; (test "foo")
-;; (test "bar")
-;; (test "123")
-;; (test "xdoc::bar)")
-;; (test "xdoc::|foo|)")
-;; (test "xdoc::bar12 ")
-;; (test ":foo)")
-;; (test ":|foo|)")
-;; (test ":")
-;; (test ":||")
-;; (test "||:")
-;; (test "::|foo|)")
-;; (test "acl2:::bar)")
-;; (test "acl2::bar)")
-;; (test "acl2::bar:")
-;; (test "acl2::bar|:|)")
-
-(defun read-literal (x n xl chars) ;; ==> (MV SUCCESSP N-PRIME)
-  ;; Try to read CHARS, verbatim.
-  (declare (type string x))
-  (cond ((= n xl)
-         (mv (atom chars) n))
-        ((consp chars)
-         (if (eql (char x n) (car chars))
-             (read-literal x (+ n 1) xl (cdr chars))
-           (mv nil n)))
-        (t
-         (mv t n))))
-
-(defun read-through-some-char-aux (x n xl chars acc) ;; ==> (MV SUCCESSP STRING N-PRIME)
-  (declare (type string x))
-  (if (= xl n)
-      (mv nil (reverse (coerce acc 'string)) n)
-    (let ((charN (char x n)))
-      (if (member charN chars)
-          (mv t (reverse (coerce (cons charN acc) 'string)) n)
-        (read-through-some-char-aux x (+ 1 n) xl chars (cons charN acc))))))
-
-(defun read-through-some-char (x n xl chars)
-  ;; Try to read until one of CHARS is found
-  (declare (type string x))
-  (read-through-some-char-aux x n xl chars nil))
-
-(defun skip-past-ws (x n xl) ;; ==> N-PRIME
-  (declare (type string x))
-  (cond ((= xl n)
-         n)
-        ((member (char x n) '(#\Space #\Tab #\Newline #\Page))
-         (skip-past-ws x (+ 1 n) xl))
-        (t
-         n)))
-
-(defun parse-directive (x n xl base-pkg) ;; ==> (MV ERROR COMMAND ARG N-PRIME)
-  ;; Every directive has the form @(command arg)
-  ;; Where command and arg are symbols.
-  ;; We assume @( has just been read, and N is now pointing right after the open paren.
-  (declare (type string x))
-  (b* ((n                    (skip-past-ws x n xl))
-       ((mv error command n) (parse-symbol x n xl 'xdoc))
-       ((when error)
-        (mv error nil nil n))
-       (n                    (skip-past-ws x n xl))
-       ((mv error arg n)     (parse-symbol x n xl base-pkg)))
-      (cond
-       ;; Some error parsing arg.  Add a little more context.
-       (error (mv (concatenate 'string "In " (symbol-name command) " directive: " error)
-                  nil nil n))
-
-       ;; Ends with ), good.
-       ((and (< n xl)
-             (eql (char x n) #\)))
-        (mv nil command arg (+ n 1)))
-
-       (t
-        (mv (concatenate 'string "In " (symbol-name command) " directive, expected ) after "
-                         (symbol-name arg)
-                         ". Near " (error-context x n xl) ".")
-            nil nil n)))))
-
-;; (let ((x "body foo)"))
-;;   (parse-directive x 0 (length x) 'acl2::foo))
-
-;; (let ((x "body foo) bar"))
-;;   (parse-directive x 0 (length x) 'acl2::foo))
-
-;; (let ((x "body xdoc::foo) bar"))
-;;   (parse-directive x 0 (length x) 'acl2::foo))
-
-;; (let ((x "xdoc::body xdoc::foo) bar"))
-;;   (parse-directive x 0 (length x) 'acl2::foo))
-
-;; (let ((x "acl2::body xdoc::foo) bar"))
-;;   (parse-directive x 0 (length x) 'acl2::foo))
-
-;; (let ((x "acl2::body)xdoc::foo) bar"))
-;;   (parse-directive x 0 (length x) 'acl2::foo))
-
-
-
-
-; -------------- Executing Directives ---------------------------
-
-(defun process-url-directive (arg state acc) ;; ===> (MV ACC STATE)
-
-; @(url foo) just expands into the file name for foo.
-
-  (b* ((acc            (file-name-mangle arg acc)))
-      (mv acc state)))
-
-
-(defun process-sym-directive (arg base-pkg state acc) ;; ===> (MV ACC STATE)
-
-; @(sym foo) just expands into the standard name mangling for foo
-
-  (b* ((acc            (sym-mangle arg base-pkg acc)))
-      (mv acc state)))
-
-
-(defun process-sym-cap-directive (arg base-pkg state acc) ;; ===> (MV ACC STATE)
-
-; @(csym foo) just expands into the standard capitalized name mangling for foo
-
-  (b* ((acc            (sym-mangle-cap arg base-pkg acc)))
-      (mv acc state)))
-
-
-(defun process-see-directive (arg base-pkg state acc) ;; ===> (MV ACC STATE)
-
-; @(see foo) just expands into a link with a lowercase name.
-
-  (b* ((acc            (str::revappend-chars "<see topic=\"" acc))
-       (acc            (file-name-mangle arg acc))
-       (acc            (str::revappend-chars "\">" acc))
-       (acc            (sym-mangle arg base-pkg acc))
-       (acc            (str::revappend-chars "</see>" acc)))
-      (mv acc state)))
-
-
-(defun process-see-cap-directive (arg base-pkg state acc) ;; ===> (MV ACC STATE)
-
-; @(csee foo) just expands into a link with a capitalized name.
-
-  (b* ((acc            (str::revappend-chars "<see topic=\"" acc))
-       (acc            (file-name-mangle arg acc))
-       (acc            (str::revappend-chars "\">" acc))
-       (acc            (sym-mangle-cap arg base-pkg acc))
-       (acc            (str::revappend-chars "</see>" acc)))
-      (mv acc state)))
-
-
-(defconst *xdoc-link-file-message*
-  "; This is an XDOC Link file.
-; Ordinarily, you should not see this file.
-;
-; If you are viewing this file in a web browser, you probably
-; have not configured your web browser to send .xdoc-link files
-; to Emacs.
-;
-;   (Or, if you have already done that, but you accessed this
-;    file through a web server, the server may just not be
-;    assigning .xdoc-link files the appropriate MIME type.)
-;
-; If you are viewing this file in Emacs, you probably have not
-; loaded xdoc.el from the xdoc/ directory.
-;
-; Please see the XDOC manual for more information.")
-
-(defun process-srclink-directive (arg dir state acc) ;; ===> (MV ACC STATE)
-
-; We do two things:
-;
-;   1. Extend acc with a srclink tag, and
-;
-;   2. Write a .xdoc-link file to dir for this tag.
-;
-; This is kind of ugly in that we may write the same .xdoc-link file many
-; times, but this doesn't seem to practically be a problem.
-;
-; Our emacs linking mechanism is slightly broken, in that all we can tell emacs
-; is the name of a symbol to look for using its tags mechanism.  We are hoping
-; that:
-;
-;   1. The user has the appropriate TAGS tables set up (reasonable),
-;
-;   2. The symbol is actually defined in a source file somewhere, instead of
-;      being introduced by a macro or something, and
-;
-;   3. The symbol is not defined in multiple packages, so that the user will be
-;      taken to the right source file.  (That is, we can't tell emacs something
-;      like "foo::bar", because it doesn't understand (in-package ...); We can
-;      only tell it to search for bar.)
-;
-; Whether or not #2 and #3 hold is a total crap-shoot, and we're basically
-; hoping that most of the time find-tag will take them to the right place.
-
-  (b* ((shortname (coerce (string-downcase (symbol-name arg)) 'list))
-       (filename  (concatenate 'string
-                               (reverse (coerce (file-name-mangle arg nil) 'string))
-                               ".xdoc-link"))
-
-       (acc (str::revappend-chars "<srclink file=\"" acc))
-       (acc (str::revappend-chars filename acc))
-       (acc (str::revappend-chars "\">" acc))
-       (acc (simple-html-encode-chars shortname acc))
-       (acc (str::revappend-chars "</srclink>" acc))
-
-       (fullpath           (acl2::extend-pathname dir filename state))
-       ((mv channel state) (open-output-channel fullpath :character state))
-       (state (princ$ *xdoc-link-file-message* channel state))
-       (state (newline channel state))
-       (state (newline channel state))
-       (state (princ$ (coerce shortname 'string) channel state))
-       (state (newline channel state))
-       (state (close-output-channel channel state)))
-      (mv acc state)))
-
-(defun process-body-directive (arg state acc) ;; ===> (MV ACC STATE)
-
-; @(body foo) -- look up the body and pretty-print it in a <code> block.
-
-  (b* ((body           (get-body arg (w state)))
-       (acc            (str::revappend-chars "<code>" acc))
-       ((mv acc state) (fmt-to-chars-and-encode "~x0"
-                                                (list (cons #\0 body))
-                                                state acc))
-       (acc            (str::revappend-chars "</code>" acc)))
-      (mv acc state)))
-
-(defun process-def-directive (arg dir state acc) ;; ===> (MV ACC STATE)
-
-; @(def foo) -- look up the definition for foo, pretty-print it in a <code>
-; block, along with a source-code link.
-
-  (b* ((def            (get-def arg (w state)))
-       (acc            (str::revappend-chars "<p><b>Definition: </b>" acc))
-       ((mv acc state) (process-srclink-directive arg dir state acc))
-       (acc            (str::revappend-chars "</p>" acc))
-       (acc            (str::revappend-chars "<code>" acc))
-       ((mv acc state) (fmt-to-chars-and-encode "~x0"
-                                                (list (cons #\0 def))
-                                                state acc))
-       (acc            (str::revappend-chars "</code>" acc)))
-      (mv acc state)))
-
-(defun process-gdef-directive (arg base-pkg state acc) ;; ===> (MV ACC STATE)
-
-; @(gdef foo) -- Look up the definition for foo, pretty-print it as in @def,
-; but don't use a source-code link because this is a "Generated Definition" for
-; which a tags-search will probably fail.
-
-  (b* ((def            (get-def arg (w state)))
-       (acc            (str::revappend-chars "<p><b>Definition: </b>" acc))
-       (acc            (sym-mangle arg base-pkg acc))
-       (acc            (str::revappend-chars "</p>" acc))
-       (acc            (str::revappend-chars "<code>" acc))
-       ((mv acc state) (fmt-to-chars-and-encode "~x0"
-                                                (list (cons #\0 def))
-                                                state acc))
-       (acc            (str::revappend-chars "</code>" acc)))
-      (mv acc state)))
-
-(defun process-thm-directive (arg dir state acc) ;; ===> (MV ACC STATE)
-
-; @(thm foo) -- Look up the theorem named foo, and pretty-print its event along
-; with a source link.
-
-  (b* ((theorem        (get-theorem arg (w state)))
-       (acc            (str::revappend-chars "<p><b>Theorem: </b>" acc))
-       ((mv acc state) (process-srclink-directive arg dir state acc))
-       (acc            (str::revappend-chars "</p>" acc))
-       (acc            (str::revappend-chars "<code>" acc))
-       ((mv acc state) (fmt-to-chars-and-encode "~x0"
-                                                (list (cons #\0 theorem))
-                                                state acc))
-       (acc            (str::revappend-chars "</code>" acc)))
-      (mv acc state)))
-
-(defun process-gthm-directive (arg base-pkg state acc) ;; ===> (MV ACC STATE)
-
-; @(gthm foo) -- Like @(thm foo), but don't provide a source link since this is
-; a generated theorem.
-
-  (b* ((theorem        (get-theorem arg (w state)))
-       (acc            (str::revappend-chars "<p><b>Theorem: </b>" acc))
-       (acc            (sym-mangle arg base-pkg acc))
-       (acc            (str::revappend-chars "</p>" acc))
-       (acc            (str::revappend-chars "<code>" acc))
-       ((mv acc state) (fmt-to-chars-and-encode "~x0"
-                                                (list (cons #\0 theorem))
-                                                state acc))
-       (acc            (str::revappend-chars "</code>" acc)))
-      (mv acc state)))
-
-(defun process-formals-directive (arg state acc) ;; ===> (MV ACC STATE)
-
-; @(formals foo) -- just find the formals for foo and print them without any
-; extra formatting.
-
-  (b* ((formals        (get-formals arg (w state)))
-       ((mv acc state) (fmt-to-chars-and-encode "~x0"
-                                                (list (cons #\0 formals))
-                                                state acc)))
-      (mv acc state)))
-
-(defun process-call-directive (arg state acc) ;; ===> (MV ACC STATE)
-
-; @(call foo) -- find the formals to foo and insert <tt>(foo x y z)</tt>.
-; BOZO consider adding an emacs link.
-
-  (b* ((formals        (get-formals arg (w state)))
-       (call           (cons arg formals))
-       (acc            (str::revappend-chars "<tt>" acc))
-       ((mv acc state) (fmt-to-chars-and-encode "~x0"
-                                                (list (cons #\0 call))
-                                                state acc))
-       (acc            (str::revappend-chars "</tt>" acc)))
-      (mv acc state)))
-
-(defun process-ccall-directive (arg state acc) ;; ===> (MV ACC STATE)
-
-; @(ccall foo) -- "code call" is like @(call foo), but uses <code> instead
-; of <tt> tags.
-
-  (b* ((formals        (get-formals arg (w state)))
-       (call           (cons arg formals))
-       (acc            (str::revappend-chars "<code>" acc))
-       ((mv acc state) (fmt-to-chars-and-encode "~x0"
-                                                (list (cons #\0 call))
-                                                state acc))
-       (acc            (str::revappend-chars "</code>" acc)))
-      (mv acc state)))
-
-(defun process-measure-directive (arg state acc) ;; ===> (MV ACC STATE)
-
-; @(measure foo) -- find the measure for foo and print it without any extra
-; formatting.
-
-  (b* ((measure        (get-measure arg (w state)))
-       ((mv acc state) (fmt-to-chars-and-encode "~x0"
-                                                (list (cons #\0 measure))
-                                                state acc)))
-      (mv acc state)))
-
-
-(defun process-directive (command arg dir base-pkg state acc) ;; ===> (MV ACC STATE)
-
-; Command and Arg are the already-parsed symbols we have read from the
-; documentation string.  Carry out whatever directive we've been asked to do.
-; DIR is the output dir.  Acc is the accumulator for our output characters.
-
-  (case command
-    (def       (process-def-directive arg dir state acc))
-    (thm       (process-thm-directive arg dir state acc))
-    (srclink   (process-srclink-directive arg dir state acc))
-    (gdef      (process-gdef-directive arg base-pkg state acc))
-    (gthm      (process-gthm-directive arg base-pkg state acc))
-    (body      (process-body-directive arg state acc))
-    (formals   (process-formals-directive arg state acc))
-    (measure   (process-measure-directive arg state acc))
-    (call      (process-call-directive arg state acc))
-    (ccall     (process-ccall-directive arg state acc))
-    (url       (process-url-directive arg state acc))
-    (see       (process-see-directive arg base-pkg state acc))
-    (csee      (process-see-cap-directive arg base-pkg state acc))
-    (sym       (process-sym-directive arg base-pkg state acc))
-    (csym      (process-sym-cap-directive arg base-pkg state acc))
-    (otherwise
-     (prog2$
-      (cw "; xdoc error: unknown directive ~x0.~%" command)
-      (let* ((acc (str::revappend-chars "[[ unknown directive " acc))
-             (acc (str::revappend-chars (symbol-name command) acc))
-             (acc (str::revappend-chars "]]" acc)))
-        (mv acc state))))))
-
-
-(defun preprocess-aux (x n xl dir base-pkg state acc) ;; ==> (MV ACC STATE)
-  (declare (type string x))
-
-; Main preprocessor loop.  Read from the string and accumulate the result into
-; acc, expanding away any preprocessor directives.
-
-  (if (= n xl)
-      (mv acc state)
-    (let ((char (char x n)))
-      (if (eql char #\@)
-          (cond ((and (< (+ n 1) xl)
-                      (eql (char x (+ n 1)) #\@))
-                 ;; @@ --> @
-                 (preprocess-aux x (+ n 2) xl dir base-pkg state (cons #\@ acc)))
-
-                ((and (< (+ n 1) xl)
-                      (eql (char x (+ n 1)) #\())
-                 ;; @( --> directive
-                 (b* (((mv error command arg n) (parse-directive x (+ n 2) xl base-pkg))
-                      ((when error)
-                       (prog2$ (cw "; xdoc error: ~x0.~%" error)
-                               (mv acc state)))
-                      ((mv acc state)
-                       (process-directive command arg dir base-pkg state acc)))
-                     (preprocess-aux x n xl dir base-pkg state acc)))
-
-                (t
-                 ;; @ sign in some other context.
-                 (preprocess-aux x (+ n 1) xl dir base-pkg state (cons #\@ acc))))
-        (preprocess-aux x (+ n 1) xl dir base-pkg state (cons char acc))))))
-
-(defun preprocess-main (x dir base-pkg state acc)
-  (declare (type string x))
-  (b* ((current-pkg    (acl2::f-get-global 'current-package state))
-       ;; Temporarily make "fmt" print as if it's in base-pkg.
-       ((mv & & state) (acl2::set-current-package (symbol-package-name base-pkg) state))
-       ((mv acc state) (preprocess-aux x 0 (length x) dir base-pkg state acc))
-       ;; Restore base-pkg for whoever called us.
-       ((mv & & state) (acl2::set-current-package current-pkg state)))
-      (mv acc state)))
-
-
 
 
 
@@ -836,12 +163,12 @@
 
 (mutual-recursion
 
- (defun make-hierarchy-aux (path dir base-pkg all id acc state)
+ (defun make-hierarchy-aux (path dir index-pkg all id acc state)
 
 ; - Path is our current location in the hierarchy, and is used to avoid loops.
 ;   (The first element in path is the current topic we are on.)
 ;
-; - Base-pkg is just used for symbol printing
+; - Index-pkg is just used for symbol printing.
 ;
 ; - All is the list of all xdoc documentation topics.
 ;
@@ -867,7 +194,8 @@
           (mv acc id state)))
 
         (topic (find-topic name all))
-        (short (cdr (assoc :short topic)))
+        (short    (cdr (assoc :short topic)))
+        (base-pkg (cdr (assoc :base-pkg topic)))
 
         (acc (str::revappend-chars "<hindex topic=\"" acc))
         (acc (file-name-mangle name acc))
@@ -879,7 +207,7 @@
         (acc (cons #\Newline acc))
 
         (acc (str::revappend-chars "<hindex_name>" acc))
-        (acc (sym-mangle-cap name base-pkg acc))
+        (acc (sym-mangle-cap name index-pkg acc))
         (acc (str::revappend-chars "</hindex_name>" acc))
         (acc (cons #\Newline acc))
 
@@ -898,13 +226,13 @@
 
         (id   (+ id 1))
         ((mv acc id state)
-         (make-hierarchy-list-aux children path dir base-pkg all id acc state))
+         (make-hierarchy-list-aux children path dir index-pkg all id acc state))
         (acc (str::revappend-chars "</hindex_children>" acc))
         (acc (str::revappend-chars "</hindex>" acc))
         (acc (cons #\Newline acc)))
        (mv acc id state)))
 
- (defun make-hierarchy-list-aux (children path dir base-pkg all id acc state)
+ (defun make-hierarchy-list-aux (children path dir index-pkg all id acc state)
 
 ; - Children are the children of this path.
 ; - Path is our current location in the hierarchy.
@@ -912,12 +240,12 @@
    (if (atom children)
        (mv acc id state)
      (b* (((mv acc id state)
-           (make-hierarchy-aux (cons (car children) path) dir base-pkg all id acc state))
+           (make-hierarchy-aux (cons (car children) path) dir index-pkg all id acc state))
           ((mv acc id state)
-           (make-hierarchy-list-aux (cdr children) path dir base-pkg all id acc state)))
+           (make-hierarchy-list-aux (cdr children) path dir index-pkg all id acc state)))
          (mv acc id state)))))
 
-(defun save-hierarchy (x dir base-pkg state)
+(defun save-hierarchy (x dir index-pkg state)
 
 ; X is all topics.  We assume all parents are normalized.
 
@@ -925,13 +253,13 @@
        (acc   nil)
        (acc   (str::revappend-chars "<?xml version=\"1.0\" encoding=\"UTF-8\"?>" acc))
        (acc   (cons #\Newline acc))
-       (acc   (str::revappend-chars "<?xml-stylesheet type=\"text/xsl\" href=\"xdoc-to-dynamic-html.xsl\"?>" acc))
+       (acc   (str::revappend-chars "<?xml-stylesheet type=\"text/xsl\" href=\"xml-topic-index.xsl\"?>" acc))
        (acc   (cons #\Newline acc))
        (acc   (str::revappend-chars "<page>" acc))
        (acc   (cons #\Newline acc))
        (acc   (str::revappend-chars "<hindex_root>" acc))
        (acc   (cons #\Newline acc))
-       ((mv acc & state) (make-hierarchy-list-aux roots nil dir base-pkg x 0 acc state))
+       ((mv acc & state) (make-hierarchy-list-aux roots nil dir index-pkg x 0 acc state))
        (acc   (str::revappend-chars "</hindex_root>" acc))
        (acc   (cons #\Newline acc))
        (acc   (str::revappend-chars "</page>" acc))
@@ -1004,7 +332,7 @@
   (b* ((acc nil)
        (acc (str::revappend-chars "<?xml version=\"1.0\" encoding=\"UTF-8\"?>" acc))
        (acc (cons #\Newline acc))
-       (acc (str::revappend-chars "<?xml-stylesheet type=\"text/xsl\" href=\"xdoc-to-dynamic-html.xsl\"?>" acc))
+       (acc (str::revappend-chars "<?xml-stylesheet type=\"text/xsl\" href=\"xml-full-index.xsl\"?>" acc))
        (acc (cons #\Newline acc))
        (acc (str::revappend-chars "<page>" acc))
        (acc (cons #\Newline acc))
@@ -1044,6 +372,7 @@
         (t
          (gather-topics names (cdr all-topics)))))
 
+
 (defun preprocess-topic (x all-topics dir state)
   (b* ((name     (cdr (assoc :name x)))
        (base-pkg (cdr (assoc :base-pkg x)))
@@ -1068,7 +397,7 @@
        (acc    nil)
        (acc    (str::revappend-chars "<?xml version=\"1.0\" encoding=\"UTF-8\"?>" acc))
        (acc    (cons #\Newline acc))
-       (acc    (str::revappend-chars "<?xml-stylesheet type=\"text/xsl\" href=\"xdoc-to-dynamic-html.xsl\"?>" acc))
+       (acc    (str::revappend-chars "<?xml-stylesheet type=\"text/xsl\" href=\"xml-topic.xsl\"?>" acc))
        (acc    (cons #\Newline acc))
        (acc    (str::revappend-chars "<page>" acc))
        (acc    (str::revappend-chars "<topic name=\"" acc))
@@ -1076,12 +405,36 @@
        (acc    (str::revappend-chars "\">" acc))
        (acc    (cons #\Newline acc))
        (acc    (add-parents parents base-pkg acc))
+       (acc    (cons #\Newline acc))
        (acc    (str::revappend-chars "<short>" acc))
-       ((mv acc state) (preprocess-main short dir base-pkg state acc))
+
+       ;; Previously: ((mv acc state) (preprocess-main short dir base-pkg state acc))
+
+       ((mv short-acc state) (preprocess-main short dir base-pkg state nil))
+       (short-str  (reverse (coerce short-acc 'string)))
+       (acc        (append short-acc acc))
+       ((mv err &) (parse-xml short-str))
+       (- (or (not err)
+              (acl2::progn$
+               (cw "~|~%WARNING: problem with :short in topic ~x0:~%" name)
+               (cw-princ$ err)
+               (cw "~%~%"))))
+
        (acc    (str::revappend-chars "</short>" acc))
        (acc    (cons #\Newline acc))
        (acc    (str::revappend-chars "<long>" acc))
-       ((mv acc state) (preprocess-main long dir base-pkg state acc))
+
+       ;; Previously: ((mv acc state) (preprocess-main long dir base-pkg state acc))
+       ((mv long-acc state) (preprocess-main long dir base-pkg state nil))
+       (long-str (reverse (coerce long-acc 'string)))
+       (acc      (append long-acc acc))
+       ((mv err &) (parse-xml long-str))
+       (- (or (not err)
+              (acl2::progn$
+               (cw "~|~%WARNING: problem with :long in topic ~x0:~%" name)
+               (cw-princ$ err)
+               (cw "~%~%"))))
+
        (acc    (str::revappend-chars "</long>" acc))
        (acc    (cons #\Newline acc))
 
@@ -1119,14 +472,6 @@
 
 
 
-
-
-
-
-(make-event
- (let ((cbd (cbd)))
-   (value `(defconst *xdoc-root-dir* ',cbd))))
-
 (defun save-success-file (ntopics dir state)
   (b* ((file           (acl2::extend-pathname dir "success.txt" state))
        ((mv out state) (open-output-channel file :character state))
@@ -1136,59 +481,67 @@
        (state          (close-output-channel out state)))
       state))
 
+(defun prepare-dir (dir state)
+  (b* (((unless (stringp dir))
+        (prog2$ (er hard? 'prepare-dir "Dir must be a string, but is: ~x0.~%" dir)
+                state))
+       (- (cw "; Preparing directory ~s0.~%" dir))
+       (dir/xml     (acl2::extend-pathname dir "xml" state))
+       (state       (mkdir dir state))
+       (state       (mkdir dir/xml state))
+
+;;       (dir/support (acl2::extend-pathname dir "support" state))
+;;       (state       (mkdir dir/support state))
+
+       (xdoc/support (acl2::extend-pathname *xdoc-dir* "support" state))
+
+       ;; We copy support/Makefile-trans to dir/Makefile.  The "-trans" part of
+       ;; its name is just to prevent people from thinking they can type "make"
+       ;; in the support directory to accomplish anything.
+       (Makefile-trans (acl2::extend-pathname xdoc/support "Makefile-trans" state))
+       (Makefile-out   (acl2::extend-pathname dir "Makefile" state))
+       (state   (stupid-copy-file Makefile-trans Makefile-out state))
+
+       (state   (stupid-copy-files xdoc/support
+                                   (list "xdoc.css"
+                                         "xdoc.js"
+                                         "plus.png"
+                                         "minus.png"
+                                         "leaf.png"
+                                         "text-topic.xsl"
+                                         "html-core.xsl"
+                                         "html-topic.xsl"
+                                         "html-full-index.xsl"
+                                         "html-brief-index.xsl"
+                                         "html-topic-index.xsl"
+                                         "xml-topic.xsl"
+                                         "xml-topic-index.xsl"
+                                         "xml-full-index.xsl")
+                                   dir/xml state))
+       (state   (stupid-copy-files xdoc/support
+                                   (list "frames2.html"
+                                         "frames3.html"
+                                         "preview.html")
+                                   dir state)))
+    state))
+
 (defun save-topics (x dir index-pkg state)
-  (cond ((not (stringp dir))
-         (prog2$ (er hard? 'save-topics "Dir must be a string, but is: ~x0.~%" dir)
-                 state))
-        ((atom x)
-         (prog2$ (cw "; xdoc note: no topics are documented.~%")
-                 state))
-        (t
-         (b* ((-        (cw "; Copying skeleton files~%"))
-              (state    (time$ (stupid-copy-files *xdoc-root-dir*
-                                                  (list "Makefile-trans"
-                                                        "xdoc.css"
-                                                        "xdoc.js"
-                                                        "xdoc-to-text.xsl"
-                                                        "frames.html"
-                                                        "xdoc-to-html-aux.xsl"
-                                                        "xdoc-to-full-index.xsl"
-                                                        "xdoc-to-brief-index.xsl"
-                                                        "xdoc-to-dynamic-html.xsl"
-                                                        "xdoc-to-static-html.xsl"
-                                                        "xdoc-to-topic-index.xsl"
-                                                        "plus.png"
-                                                        "minus.png"
-                                                        "leaf.png")
-                                                  dir state)))
-              ;; Note: generate the index after the topic files, so that errors
-              ;; in short messages will be seen there.
-              (x        (normalize-parents-list x))
-              (-        (cw "; Preprocess and save ~x0 topics.~%" (len x)))
-              (state    (time$ (save-topics-aux x x dir state)))
-              (-        (cw "; Generate index.xml"))
-              (state    (time$ (save-index x dir index-pkg state)))
-              (-        (cw "; Generate topics.xml"))
-              (state    (time$ (save-hierarchy x dir index-pkg state)))
-              (-        (cw "; Save success.txt"))
-              (state    (save-success-file (len x) dir state)))
-             state))))
+  (b* ((state (prepare-dir dir state))
+       (dir   (acl2::extend-pathname dir "xml" state))
+       (- (cw "; Processing ~x0 topics.~%" (len x)))
+       ;; Note: generate the index after the topic files, so that
+       ;; errors in short messages will be seen there.
+       (x      (time$ (normalize-parents-list x)
+                      :msg "; Normalizing parents: ~st sec, ~sa bytes~%"
+                      :mintime 1/2))
+       (state  (time$ (save-topics-aux x x dir state)
+                      :msg "; Saving topics: ~st sec, ~sa bytes~%"
+                      :mintime 1/2))
+       (state  (time$ (save-index x dir index-pkg state)
+                      :msg "; Saving flat index: ~st sec, ~sa bytes~%"
+                      :mintime 1/2))
+       (state  (time$ (save-hierarchy x dir index-pkg state)
+                      :msg "; Saving hierarchical index: ~st sec, ~sa bytes~%"))
+       (state  (save-success-file (len x) dir state)))
+    state))
 
-
-
-(defun unsound-all-xdoc-topics (world)
-  (declare (xargs :mode :program)
-           (ignore world))
-  (er hard? 'unsound-all-xdoc-topics
-      "Unsound-all-xdoc-topics not yet defined."))
-
-(defttag xdoc-raw)
-(acl2::progn!
- (set-raw-mode t)
- (defun unsound-all-xdoc-topics (world)
-   (append (get-xdoc-table world)
-           *raw-xdoc-list*)))
-(defttag nil)
-
-(defmacro save (dir &key (index-pkg 'acl2::foo))
-  `(save-topics (unsound-all-xdoc-topics (w state)) ,dir ',index-pkg state))
