books/xdoc/support/html-core.xsl
@@ -1,0 +1,186 @@
+<?xml version="1.0" encoding="UTF-8"?>
+<xsl:stylesheet version="1.0" xmlns:xsl="http://www.w3.org/1999/XSL/Transform">
+
+<!--
+
+; XDOC Documentation System for ACL2
+; Copyright (C) 2009-2010 Centaur Technology
+;
+; Contact:
+;   Centaur Technology Formal Verification Group
+;   7600-C N. Capital of Texas Highway, Suite 300, Austin, TX 78731, USA.
+;   http://www.centtech.com/
+;
+; This program is free software; you can redistribute it and/or modify it under
+; the terms of the GNU General Public License as published by the Free Software
+; Foundation; either version 2 of the License, or (at your option) any later
+; version.  This program is distributed in the hope that it will be useful but
+; WITHOUT ANY WARRANTY; without even the implied warranty of MERCHANTABILITY or
+; FITNESS FOR A PARTICULAR PURPOSE.  See the GNU General Public License for
+; more details.  You should have received a copy of the GNU General Public
+; License along with this program; if not, write to the Free Software
+; Foundation, Inc., 51 Franklin Street, Suite 500, Boston, MA 02110-1335, USA.
+;
+; Original author: Jared Davis <jared@centtech.com>
+
+  html-core.xsl - main conversion from xdoc markup to html
+
+-->
+
+<xsl:template match="page">
+  <html>
+  <head>
+    <title><xsl:value-of select="@name"/></title>
+    <link rel="stylesheet" type="text/css" href="xdoc.css"/>
+    <script type="text/javascript" src="xdoc.js"/>
+  </head>
+  <body class="body_normal">
+  <xsl:apply-templates/>
+  </body>
+  </html>
+</xsl:template>
+
+<xsl:template match="index">
+  <h3><xsl:value-of select="@title"/></h3>
+  <dl class="index_dl">
+  <xsl:for-each select="index_entry">
+    <xsl:sort select="index_head/see" />
+    <dt class="index_dt"><xsl:apply-templates select="index_head"/></dt>
+    <dd class="index_dd"><xsl:apply-templates select="index_body"/></dd>
+  </xsl:for-each>
+  </dl>
+</xsl:template>
+
+<xsl:template match="topic">
+  <h1><xsl:value-of select="@name"/></h1>
+  <xsl:apply-templates/>
+</xsl:template>
+
+<xsl:template match="hindex_root">
+  <ul class="hindex"><xsl:apply-templates/></ul>
+</xsl:template>
+
+<xsl:template match="hindex_children">
+  <xsl:choose>
+    <xsl:when test="@kind='hide'">
+	<ul class="hindex" id="{@id}" style="display: none">
+	<xsl:apply-templates/>
+	</ul>
+    </xsl:when>
+
+    <xsl:otherwise>
+	<ul class="hindex" id="{@id}">
+	<xsl:apply-templates/>
+	</ul>
+    </xsl:otherwise>
+  </xsl:choose>
+</xsl:template>
+
+<xsl:template match="hindex_short">
+</xsl:template>
+
+<xsl:template match="hindex_name">
+</xsl:template>
+
+<xsl:template match="short">
+  <p><xsl:apply-templates/></p>
+</xsl:template>
+
+<xsl:template match="srclink">
+  <a href="{@file}" class="srclink" title="Find-Tag in Emacs">
+    <xsl:apply-templates/>
+  </a>
+</xsl:template>
+
+<xsl:template match="code">
+  <pre class="code"><xsl:apply-templates/></pre>
+</xsl:template>
+
+<xsl:template match="box">
+  <div class="box"><xsl:apply-templates/></div>
+</xsl:template>
+
+<xsl:template match="p">
+  <p><xsl:apply-templates/></p>
+</xsl:template>
+
+<xsl:template match="br">
+  <xsl:apply-templates/><br/>
+</xsl:template>
+
+<xsl:template match="a">
+  <a href="{@href}">
+    <xsl:value-of select="."/>
+  </a>
+</xsl:template>
+
+<xsl:template match="b">
+  <b><xsl:apply-templates/></b>
+</xsl:template>
+
+<xsl:template match="i">
+  <i><xsl:apply-templates/></i>
+</xsl:template>
+
+<xsl:template match="color">
+  <font color="{@rgb}"><xsl:apply-templates/></font>
+</xsl:template>
+
+<xsl:template match="sf">
+  <span class="sf"><xsl:apply-templates/></span>
+</xsl:template>
+
+<xsl:template match="u">
+  <u><xsl:apply-templates/></u>
+</xsl:template>
+
+<xsl:template match="tt">
+  <span class="tt"><xsl:apply-templates/></span>
+</xsl:template>
+
+<xsl:template match="ul">
+  <ul><xsl:apply-templates/></ul>
+</xsl:template>
+
+<xsl:template match="ol">
+  <ol><xsl:apply-templates/></ol>
+</xsl:template>
+
+<xsl:template match="li">
+  <li><xsl:apply-templates/></li>
+</xsl:template>
+
+<xsl:template match="dl">
+  <dl><xsl:apply-templates/></dl>
+</xsl:template>
+
+<xsl:template match="dt">
+  <dt><xsl:apply-templates/></dt>
+</xsl:template>
+
+<xsl:template match="dd">
+  <dd><xsl:apply-templates/></dd>
+</xsl:template>
+
+<xsl:template match="h1">
+  <h1><xsl:apply-templates/></h1>
+</xsl:template>
+
+<xsl:template match="h2">
+  <h2><xsl:apply-templates/></h2>
+</xsl:template>
+
+<xsl:template match="h3">
+  <h3><xsl:apply-templates/></h3>
+</xsl:template>
+
+<xsl:template match="h4">
+  <h4><xsl:apply-templates/></h4>
+</xsl:template>
+
+<xsl:template match="h5">
+  <h5><xsl:apply-templates/></h5>
+</xsl:template>
+
+
+</xsl:stylesheet>
